Make Impl/Common files work with Dafny 3.0.0

ironfleet/src/Dafny/Distributed/Impl/Common/GenericMarshalling.i.dfy
@@ -1,4 +1,3 @@
-//include "../../../Libraries/Util/be_sequences.s.dfy"
 include "../../Common/Native/NativeTypes.s.dfy"
 include "../../Common/Collections/Maps.i.dfy"
 include "../../Common/Collections/Seqs.i.dfy"
@@ -7,13 +6,15 @@ include "Util.i.dfy"
 include "MarshallInt.i.dfy"
 
 module Common__GenericMarshalling_i {
-//import opened Util__be_sequences_s
+import opened Native__Io_s
 import opened Native__NativeTypes_s
+import opened Native__NativeTypes_i
 import opened Collections__Maps_i
 import opened Collections__Seqs_i 
 import opened Logic__Option_i
 import opened Common__Util_i
 import opened Common__MarshallInt_i
+import opened Math__power2_i
 
 datatype G = GUint64
            | GArray(elt:G)
@@ -29,1833 +30,1810 @@ datatype V = VUint64(u:uint64)
 
 predicate ValInGrammar(val:V, grammar:G)
 {
-    match val
-        case VUint64(_) => grammar.GUint64?
-        case VArray(a)  => grammar.GArray? && forall v :: v in a ==> ValInGrammar(v, grammar.elt)
-        case VTuple(t)  => grammar.GTuple? && |t| == |grammar.t|
-                              && forall i :: 0 <= i < |t| ==> ValInGrammar(t[i], grammar.t[i])
-        case VByteArray(b) => grammar.GByteArray?
-        case VCase(c, v) => grammar.GTaggedUnion? && int(c) < |grammar.cases| && ValInGrammar(v, grammar.cases[c])
+  match val
+    case VUint64(_)    => grammar.GUint64?
+    case VArray(a)     => grammar.GArray? && forall v :: v in a ==> ValInGrammar(v, grammar.elt)
+    case VTuple(t)     => grammar.GTuple? && |t| == |grammar.t| && (forall i :: 0 <= i < |t| ==> ValInGrammar(t[i], grammar.t[i]))
+    case VByteArray(b) => grammar.GByteArray?
+    case VCase(c, v)   => grammar.GTaggedUnion? && c as int < |grammar.cases| && ValInGrammar(v, grammar.cases[c])
 }
 
 // We only support reasonably sized grammars
 predicate ValidGrammar(grammar:G) 
 {
-    match grammar
-        case GUint64 => true
-        case GArray(elt) => ValidGrammar(elt)
-        case GTuple(t) => |t| < 0x1_0000_0000_0000_0000 && (forall g :: g in t ==> ValidGrammar(g))
-        case GByteArray => true
-        case GTaggedUnion(cases) => |cases| < 0x1_0000_0000_0000_0000 && (forall g :: g in cases ==> ValidGrammar(g))
+  match grammar
+    case GUint64             => true
+    case GArray(elt)         => ValidGrammar(elt)
+    case GTuple(t)           => |t| < 0x1_0000_0000_0000_0000 && (forall g :: g in t ==> ValidGrammar(g))
+    case GByteArray          => true
+    case GTaggedUnion(cases) => |cases| < 0x1_0000_0000_0000_0000 && (forall g :: g in cases ==> ValidGrammar(g))
 }
 
 // We can't encode values that are not valid
 predicate ValidVal(val:V)
 {
-    match val
-        case VUint64(_)    => true
-        case VArray(a)     => |a| < 0x1_0000_0000_0000_0000 && forall v :: v in a ==> ValidVal(v)
-        case VTuple(t)     => |t| < 0x1_0000_0000_0000_0000 && forall v :: v in t ==> ValidVal(v)
-        case VByteArray(b) => |b| < 0x1_0000_0000_0000_0000
-        case VCase(c, v) => ValidVal(v)
-
+  match val
+    case VUint64(_)    => true
+    case VArray(a)     => |a| < 0x1_0000_0000_0000_0000 && forall v :: v in a ==> ValidVal(v)
+    case VTuple(t)     => |t| < 0x1_0000_0000_0000_0000 && forall v :: v in t ==> ValidVal(v)
+    case VByteArray(b) => |b| < 0x1_0000_0000_0000_0000
+    case VCase(c, v)   => ValidVal(v)
 }
 
 function {:opaque} SeqSum(t:seq<V>) : int
-    ensures SeqSum(t) >= 0;
+  ensures SeqSum(t) >= 0
 {
-    if |t| == 0 then 0
-    else SizeOfV(t[0]) + SeqSum(t[1..])
+  if |t| == 0 then 0
+  else SizeOfV(t[0]) + SeqSum(t[1..])
 }
 
 function SizeOfV(val:V) : int
-    ensures SizeOfV(val) >= 0;
+  ensures SizeOfV(val) >= 0
 {
-    match val
-        case VUint64(_)     => 8
-        case VArray(a)      => 8 + SeqSum(a)     // 8 bytes for length
-        case VTuple(t)      => SeqSum(t)
-        case VByteArray(b)  => 8 + |b|          // 8 bytes for a length field
-        case VCase(c, v)  => 8 + SizeOfV(v)     // 8 bytes for the case identifier
+  match val
+    case VUint64(_)     => 8
+    case VArray(a)      => 8 + SeqSum(a)     // 8 bytes for length
+    case VTuple(t)      => SeqSum(t)
+    case VByteArray(b)  => 8 + |b|          // 8 bytes for a length field
+    case VCase(c, v)    => 8 + SizeOfV(v)     // 8 bytes for the case identifier
+}
+
+predicate Trigger(i:int)
+{
+  true
 }
 
 function method parse_Uint64(data:seq<byte>) : (Option<V>, seq<byte>)
-    requires |data| < 0x1_0000_0000_0000_0000;
+  requires |data| < 0x1_0000_0000_0000_0000
 {
-    if uint64(|data|) >= Uint64Size() then
-        (Some(VUint64(SeqByteToUint64(data[..Uint64Size()]))), data[Uint64Size()..])
-    else
-        (None, [])
+  if |data| as uint64 >= Uint64Size() then
+    (Some(VUint64(SeqByteToUint64(data[..Uint64Size()]))), data[Uint64Size()..])
+  else
+    (None, [])
 }
 
 method ParseUint64(data:array<byte>, index:uint64) returns (success:bool, v:V, rest_index:uint64)
-    requires data != null;
-    requires int(index) <= data.Length;
-    requires data.Length < 0x1_0000_0000_0000_0000;
-    ensures  int(rest_index) <= data.Length;
-    ensures  var (v', rest') := parse_Uint64(data[index..]);
-             var v_opt := if success then Some(v) else None();
-             v_opt == v' && data[rest_index..] == rest';
+  requires index as int <= data.Length
+  requires data.Length < 0x1_0000_0000_0000_0000
+  ensures  rest_index as int <= data.Length
+  ensures  var (v', rest') := parse_Uint64(data[index..]);
+           var v_opt := if success then Some(v) else None();
+           v_opt == v' && data[rest_index..] == rest'
 {
-    lemma_2toX();
+  lemma_2toX();
 
-    if uint64(data.Length) >= 8 && index <= uint64(data.Length) - 8 {
-    // Avoids overflow and equvalent to: if index + 8 < uint64(data.Length) {
-        var result := uint64(data[index + uint64(0)]) * 0x1_00_0000_0000_0000
-                    + uint64(data[index + uint64(1)]) * 0x1_00_0000_0000_00
-                    + uint64(data[index + uint64(2)]) * 0x1_00_0000_0000
-                    + uint64(data[index + uint64(3)]) * 0x1_00_0000_00
-                    + uint64(data[index + uint64(4)]) * 0x1_00_0000
-                    + uint64(data[index + uint64(5)]) * 0x1_00_00
-                    + uint64(data[index + uint64(6)]) * 0x1_00
-                    + uint64(data[index + uint64(7)]);
-        success := true;
-        v := VUint64(result);
-        rest_index := index + Uint64Size();
-    } else {
-        success := false;
-        rest_index := uint64(data.Length);
-    }
+  if data.Length as uint64 >= 8 && index <= (data.Length as uint64) - 8 {
+    // Avoids overflow and equvalent to: if index + 8 < (data.Length as uint64) {
+    var result := (data[index as int] as uint64) * 0x1_00_0000_0000_0000
+                  + (data[index as int + 1] as uint64) * 0x1_00_0000_0000_00
+                  + (data[index as int + 2] as uint64) * 0x1_00_0000_0000
+                  + (data[index as int + 3] as uint64) * 0x1_00_0000_00
+                  + (data[index as int + 4] as uint64) * 0x1_00_0000
+                  + (data[index as int + 5] as uint64) * 0x1_00_00
+                  + (data[index as int + 6] as uint64) * 0x1_00
+                  + (data[index as int + 7] as uint64);
+    success := true;
+    v := VUint64(result);
+    rest_index := index + Uint64Size();
+  } else {
+    success := false;
+    rest_index := data.Length as uint64;
+  }
 }
 
 function method {:opaque} parse_Array_contents(data:seq<byte>, eltType:G, len:uint64) : (Option<seq<V>>, seq<byte>)
-    requires |data| < 0x1_0000_0000_0000_0000;
-    requires ValidGrammar(eltType);
-    decreases eltType, 1, len;
-    ensures var (opt_seq, rest) := parse_Array_contents(data, eltType, len);
-            |rest| <= |data| && (opt_seq.Some? ==> forall i :: 0 <= i < |opt_seq.v| ==> ValInGrammar(opt_seq.v[i], eltType));
+  requires |data| < 0x1_0000_0000_0000_0000
+  requires ValidGrammar(eltType)
+  decreases eltType, 1, len
+  ensures  var (opt_seq, rest) := parse_Array_contents(data, eltType, len);
+           |rest| <= |data| && (opt_seq.Some? ==> forall i :: 0 <= i < |opt_seq.v| ==> ValInGrammar(opt_seq.v[i], eltType))
 {
-   if len == 0 then
-       (Some([]), data)
-   else
-       var (val, rest1) := parse_Val(data, eltType);
-       var (others, rest2) := parse_Array_contents(rest1, eltType, len - 1);
-       if !val.None? && !others.None? then
-           (Some([val.v] + others.v), rest2)
-       else
-           (None, [])
+  if len == 0 then
+    (Some([]), data)
+  else
+    var (val, rest1) := parse_Val(data, eltType);
+    var (others, rest2) := parse_Array_contents(rest1, eltType, len - 1);
+    if !val.None? && !others.None? then
+      (Some([val.v] + others.v), rest2)
+    else
+      (None, [])
 }
 
 datatype ContentsTraceStep = ContentsTraceStep(data:seq<byte>, val:Option<V>)
 
 lemma lemma_ArrayContents_helper(data:seq<byte>, eltType:G, len:uint64, v:seq<V>, trace:seq<ContentsTraceStep>)
-    requires |data| < 0x1_0000_0000_0000_0000;
-    requires ValidGrammar(eltType);
-    requires |trace| == int(len) + 1;
-    requires |v| == int(len);
-    requires forall j :: 0 <= j < |trace| ==> |trace[j].data| < 0x1_0000_0000_0000_0000;
-    requires trace[0].data == data;
-    requires forall j :: 0 < j < int(len)+1 ==> 
-                    trace[j].val  == parse_Val(trace[j-1].data, eltType).0
-                 && trace[j].data == parse_Val(trace[j-1].data, eltType).1;
-    requires forall j :: 0 < j < |trace| ==> trace[j].val.Some?;
-    requires forall j :: 0 < j < |trace| ==> v[j-1] == trace[j].val.v;
-    //requires v == ExtractValues(trace[1..]);
-    decreases len;
-    ensures  var (v', rest') := parse_Array_contents(data, eltType, len);
-             var v_opt := Some(v);
-             v_opt == v' && trace[|trace|-1].data == rest';
+  requires |data| < 0x1_0000_0000_0000_0000
+  requires ValidGrammar(eltType)
+  requires |trace| == (len as int) + 1
+  requires |v| == len as int
+  requires forall j :: 0 <= j < |trace| ==> |trace[j].data| < 0x1_0000_0000_0000_0000
+  requires trace[0].data == data
+  requires forall j :: 0 < j < (len as int) + 1 ==> 
+                 && trace[j].val  == parse_Val(trace[j-1].data, eltType).0
+                 && trace[j].data == parse_Val(trace[j-1].data, eltType).1
+  requires forall j :: 0 < j < |trace| ==> trace[j].val.Some?;
+  requires forall j :: 0 < j < |trace| ==> v[j-1] == trace[j].val.v;
+  //requires v == ExtractValues(trace[1..])
+  decreases len;
+  ensures  var (v', rest') := parse_Array_contents(data, eltType, len);
+           var v_opt := Some(v);
+           v_opt == v' && trace[|trace|-1].data == rest'
 {
-    reveal_parse_Array_contents();
-    if len == 0 {
-    } else {
-        var tuple := parse_Val(data, eltType);
-        var val, rest1 := tuple.0, tuple.1;
-        assert trace[1].data == rest1;
-        assert val.Some?;
-        assert trace[1].val == val;
-        lemma_ArrayContents_helper(rest1, eltType, len-1, v[1..], trace[1..]);
-        var tuple'' := parse_Array_contents(rest1, eltType, len-1);
-        var v'', rest'' := tuple''.0, tuple''.1;
-        var v_opt'' := Some(v[1..]);
-        assert v_opt'' == v'' && trace[1..][|trace[1..]|-1].data == rest'';
+  reveal parse_Array_contents();
+  if len == 0 {
+  } else {
+    var tuple := parse_Val(data, eltType);
+    var val, rest1 := tuple.0, tuple.1;
+    assert trace[1].data == rest1;
+    assert val.Some?;
+    assert trace[1].val == val;
+    lemma_ArrayContents_helper(rest1, eltType, len-1, v[1..], trace[1..]);
+    var tuple'' := parse_Array_contents(rest1, eltType, len-1);
+    var v'', rest'' := tuple''.0, tuple''.1;
+    var v_opt'' := Some(v[1..]);
+    assert v_opt'' == v'' && trace[1..][|trace[1..]|-1].data == rest'';
 
-        var tuple' := parse_Array_contents(data, eltType, len);
-        var v', rest' := tuple'.0, tuple'.1;
-        calc { 
-            v'; 
-            Some([val.v] + v''.v);
-            Some([val.v] + v[1..]);
-            Some([v[0]] + v[1..]);
-                { assert v == [v[0]] + v[1..]; }
-            Some(v);
-        }
-        assert rest' == rest'';
+    var tuple' := parse_Array_contents(data, eltType, len);
+    var v', rest' := tuple'.0, tuple'.1;
+    calc { 
+      v'; 
+      Some([val.v] + v''.v);
+      Some([val.v] + v[1..]);
+      Some([v[0]] + v[1..]);
+        { assert v == [v[0]] + v[1..]; }
+      Some(v);
     }
+    assert rest' == rest'';
+  }
 }
 
 lemma lemma_ArrayContents_helper_bailout(data:seq<byte>, eltType:G, len:uint64, trace:seq<ContentsTraceStep>)
-    requires |data| < 0x1_0000_0000_0000_0000;
-    requires ValidGrammar(eltType);
-    requires 1 < |trace| <= int(len) + 1;
-    //requires |v| == int(len);
-    requires forall j :: 0 <= j < |trace| ==> |trace[j].data| < 0x1_0000_0000_0000_0000;
-    requires trace[0].data == data;
-    requires forall j :: 0 < j < |trace| ==> 
-                    trace[j].val  == parse_Val(trace[j-1].data, eltType).0
-                 && trace[j].data == parse_Val(trace[j-1].data, eltType).1;
-    requires forall j :: 0 < j < |trace| - 1 ==> trace[j].val.Some?;
-    //requires forall j :: 0 < j < |trace| - 1 ==> v[j-1] == trace[j].val.v;
-    requires trace[|trace|-1].val.None?;
-    //requires v == ExtractValues(trace[1..]);
-    decreases len;
-    ensures  var (v', rest') := parse_Array_contents(data, eltType, len);
-             v'.None? && rest' == [];
+  requires |data| < 0x1_0000_0000_0000_0000
+  requires ValidGrammar(eltType)
+  requires 1 < |trace| <= (len as int) + 1
+  //requires |v| == len as int
+  requires forall j :: 0 <= j < |trace| ==> |trace[j].data| < 0x1_0000_0000_0000_0000
+  requires trace[0].data == data
+  requires forall j :: 0 < j < |trace| ==> 
+                 && trace[j].val  == parse_Val(trace[j-1].data, eltType).0
+                 && trace[j].data == parse_Val(trace[j-1].data, eltType).1
+  requires forall j :: 0 < j < |trace| - 1 ==> trace[j].val.Some?;
+  //requires forall j :: 0 < j < |trace| - 1 ==> v[j-1] == trace[j].val.v
+  requires trace[|trace|-1].val.None?
+  //requires v == ExtractValues(trace[1..])
+  decreases len
+  ensures  var (v', rest') := parse_Array_contents(data, eltType, len);
+           v'.None? && rest' == []
 {
-    reveal_parse_Array_contents();
+  reveal parse_Array_contents();
     
-    var tuple := parse_Val(data, eltType);
-    var val, rest1 := tuple.0, tuple.1;
-    if |trace| == 2 {
-        assert val.None?;
-        var tuple' := parse_Array_contents(data, eltType, len);
-        var v', rest' := tuple'.0, tuple'.1;
-        assert v'.None?;
-        assert rest' == [];
-    } else {
-        lemma_ArrayContents_helper_bailout(rest1, eltType, len-1, trace[1..]);
-    }
+  var tuple := parse_Val(data, eltType);
+  var val, rest1 := tuple.0, tuple.1;
+  if |trace| == 2 {
+    assert val.None?;
+    var tuple' := parse_Array_contents(data, eltType, len);
+    var v', rest' := tuple'.0, tuple'.1;
+    assert v'.None?;
+    assert rest' == [];
+  } else {
+    lemma_ArrayContents_helper_bailout(rest1, eltType, len-1, trace[1..]);
+  }
 }
 
 method{:timeLimitMultiplier 2} ParseArrayContents(data:array<byte>, index:uint64, eltType:G, len:uint64) 
        returns (success:bool, v:seq<V>, rest_index:uint64)
-    requires data != null;
-    requires int(index) <= data.Length;
-    requires data.Length < 0x1_0000_0000_0000_0000;
-    requires ValidGrammar(eltType);
-    decreases eltType, 1, len;
-    ensures  int(rest_index) <= data.Length;
-    ensures  var (v', rest') := parse_Array_contents(data[index..], eltType, len);
-             var v_opt := if success then Some(v) else None();
-             v_opt == v' && data[rest_index..] == rest';
-    ensures  success ==> ValidVal(VArray(v));
+  requires index as int <= data.Length
+  requires data.Length < 0x1_0000_0000_0000_0000
+  requires ValidGrammar(eltType)
+  decreases eltType, 1, len
+  ensures  rest_index as int <= data.Length
+  ensures  var (v', rest') := parse_Array_contents(data[index..], eltType, len);
+           var v_opt := if success then Some(v) else None();
+           v_opt == v' && data[rest_index..] == rest'
+  ensures  success ==> ValidVal(VArray(v))
 {
-    reveal_parse_Array_contents();
-    var vArr := new V[len];
-    ghost var g_v := [];
-    success := true;
-    var i:uint64 := 0;
-    var next_val_index:uint64 := index;
-    ghost var trace := [ContentsTraceStep(data[index..], None())];
+  reveal parse_Array_contents();
+  var vArr := new V[len];
+  ghost var g_v := [];
+  success := true;
+  var i:uint64 := 0;
+  var next_val_index:uint64 := index;
+  ghost var trace := [ContentsTraceStep(data[index..], None())];
 
-    while i < len
-        invariant 0 <= i <= len;
-        invariant index <= next_val_index <= uint64(data.Length);
-        invariant |trace| == int(i) + 1;
-        invariant |g_v| == int(i);
-        invariant vArr[..i] == g_v;
-        invariant trace[0].data == data[index..];
-        invariant forall j :: 0 <= j < int(i)+1 ==> |trace[j].data| < 0x1_0000_0000_0000_0000;
-        invariant trace[i].data == data[next_val_index..];
-        invariant forall j :: 0 < j <= i ==> trace[j].val.Some?;
-        invariant forall j :: 0 < j <= i ==> g_v[j-1] == trace[j].val.v;
-        invariant forall j :: 0 < j < int(i)+1 ==> 
-            trace[j].val  == parse_Val(trace[j-1].data, eltType).0
-         && trace[j].data == parse_Val(trace[j-1].data, eltType).1
-        invariant ValidVal(VArray(vArr[..i]));
-    {
-        var some1, val, rest1 := ParseVal(data, next_val_index, eltType);
-        ghost var step := ContentsTraceStep(data[rest1..], if some1 then Some(val) else None());
-        ghost var old_trace := trace;
-        trace := trace + [step];
-        if !some1 {
-            success := false;
-            rest_index := uint64(data.Length);
-            lemma_ArrayContents_helper_bailout(data[index..], eltType, len, trace);
-            return;
-        }
-        g_v := g_v + [val];
-        vArr[i] := val;
-        next_val_index := rest1;
-
-        i := i + 1;
+  while i < len
+    invariant 0 <= i <= len
+    invariant index <= next_val_index <= data.Length as uint64
+    invariant |trace| == (i as int) + 1
+    invariant |g_v| == i as int
+    invariant vArr[..i] == g_v
+    invariant trace[0].data == data[index..]
+    invariant forall j :: 0 <= j < (i as int)+1 ==> |trace[j].data| < 0x1_0000_0000_0000_0000
+    invariant trace[i].data == data[next_val_index..]
+    invariant forall j :: 0 < j <= i ==> trace[j].val.Some?
+    invariant forall j :: 0 < j <= i ==> g_v[j-1] == trace[j].val.v
+    invariant forall j :: 0 < j < (i as int)+1 ==>
+                    && trace[j].val  == parse_Val(trace[j-1].data, eltType).0
+                    && trace[j].data == parse_Val(trace[j-1].data, eltType).1
+    invariant ValidVal(VArray(vArr[..i]))
+  {
+    var some1, val, rest1 := ParseVal(data, next_val_index, eltType);
+    ghost var step := ContentsTraceStep(data[rest1..], if some1 then Some(val) else None());
+    ghost var old_trace := trace;
+    trace := trace + [step];
+    if !some1 {
+      success := false;
+      rest_index := data.Length as uint64;
+      lemma_ArrayContents_helper_bailout(data[index..], eltType, len, trace);
+      return;
     }
+    g_v := g_v + [val];
+    vArr[i] := val;
+    next_val_index := rest1;
 
-    success := true;
-    rest_index := next_val_index;
-    v := vArr[..];               
-    lemma_ArrayContents_helper(data[index..], eltType, len, v, trace);
+    i := i + 1;
+  }
+
+  success := true;
+  rest_index := next_val_index;
+  v := vArr[..];               
+  lemma_ArrayContents_helper(data[index..], eltType, len, v, trace);
 }
 
 function method parse_Array(data:seq<byte>, eltType:G) : (Option<V>, seq<byte>)
-    requires ValidGrammar(eltType);
-    requires |data| < 0x1_0000_0000_0000_0000;
-    decreases eltType;
-    ensures var (opt_val, rest) := parse_Array(data, eltType);
-            |rest| <= |data| && (opt_val.Some? ==> ValInGrammar(opt_val.v, GArray(eltType)));
+  requires ValidGrammar(eltType)
+  requires |data| < 0x1_0000_0000_0000_0000
+  decreases eltType
+  ensures var (opt_val, rest) := parse_Array(data, eltType);
+          |rest| <= |data| && (opt_val.Some? ==> ValInGrammar(opt_val.v, GArray(eltType)))
 {
-    var (len, rest) := parse_Uint64(data);
-    if !len.None? then
-        var (contents, remainder) := parse_Array_contents(rest, eltType, len.v.u);
-        if !contents.None? then
-            (Some(VArray(contents.v)), remainder)
-        else
-            (None, [])
+  var (len, rest) := parse_Uint64(data);
+  if !len.None? then
+    var (contents, remainder) := parse_Array_contents(rest, eltType, len.v.u);
+    if !contents.None? then
+      (Some(VArray(contents.v)), remainder)
     else
-        (None, [])
+      (None, [])
+  else
+    (None, [])
 }
 
 method ParseArray(data:array<byte>, index:uint64, eltType:G) returns (success:bool, v:V, rest_index:uint64)
-    requires data != null;
-    requires int(index) <= data.Length;
-    requires data.Length < 0x1_0000_0000_0000_0000;
-    requires ValidGrammar(eltType);
-    decreases eltType;
-    ensures  int(rest_index) <= data.Length;
-    ensures  var (v', rest') := parse_Array(data[index..], eltType);
-             var v_opt := if success then Some(v) else None();
-             v_opt == v' && data[rest_index..] == rest';
-    ensures  success ==> ValidVal(v);
+  requires index as int <= data.Length
+  requires data.Length < 0x1_0000_0000_0000_0000
+  requires ValidGrammar(eltType)
+  decreases eltType
+  ensures  rest_index as int <= data.Length
+  ensures  var (v', rest') := parse_Array(data[index..], eltType);
+           var v_opt := if success then Some(v) else None();
+           v_opt == v' && data[rest_index..] == rest'
+  ensures  success ==> ValidVal(v);
 {
-    var some1, len, rest := ParseUint64(data, index);
-    if some1 {
-        var some2, contents, remainder := ParseArrayContents(data, rest, eltType, len.u);
-        if some2 {
-            success := true;
-            v := VArray(contents);
-            rest_index := remainder;
-        } else {
-            success := false;
-            rest_index := uint64(data.Length);
-        }
+  var some1, len, rest := ParseUint64(data, index);
+  if some1 {
+    var some2, contents, remainder := ParseArrayContents(data, rest, eltType, len.u);
+    if some2 {
+      success := true;
+      v := VArray(contents);
+      rest_index := remainder;
     } else {
-        success := false;
-        rest_index := uint64(data.Length);
+      success := false;
+      rest_index := data.Length as uint64;
     }
+  } else {
+    success := false;
+    rest_index := data.Length as uint64;
+  }
 }
 
 
 function method {:opaque} parse_Tuple_contents(data:seq<byte>, eltTypes:seq<G>) : (Option<seq<V>>, seq<byte>)
-    requires |data| < 0x1_0000_0000_0000_0000;
-    requires |eltTypes| < 0x1_0000_0000_0000_0000;
-    requires forall elt :: elt in eltTypes ==> ValidGrammar(elt);
-    decreases eltTypes, 0;
-    ensures var (opt_val, rest) := parse_Tuple_contents(data, eltTypes);
-            |rest| <= |data| &&
-            (opt_val.Some? ==> (|opt_val.v| == |eltTypes|
-                              && forall i :: 0 <= i < |opt_val.v| ==> ValInGrammar(opt_val.v[i], eltTypes[i])));
+  requires |data| < 0x1_0000_0000_0000_0000
+  requires |eltTypes| < 0x1_0000_0000_0000_0000
+  requires forall elt :: elt in eltTypes ==> ValidGrammar(elt)
+  decreases eltTypes, 0
+  ensures var (opt_val, rest) := parse_Tuple_contents(data, eltTypes);
+          |rest| <= |data| &&
+          (opt_val.Some? ==> (|opt_val.v| == |eltTypes|
+                              && forall i :: 0 <= i < |opt_val.v| ==> ValInGrammar(opt_val.v[i], eltTypes[i])))
 {
-    if eltTypes == [] then
-        (Some([]), data)
+  if eltTypes == [] then
+    (Some([]), data)
+  else
+    var (val, rest1) := parse_Val(data, eltTypes[0]);
+    assert |rest1| <= |data|;
+    var (contents, rest2) := parse_Tuple_contents(rest1, eltTypes[1..]);
+    if !val.None? && !contents.None? then
+      (Some([val.v] + contents.v), rest2)
     else
-        var (val, rest1) := parse_Val(data, eltTypes[uint64(0)]);
-        assert |rest1| <= |data|;
-        var (contents, rest2) := parse_Tuple_contents(rest1, eltTypes[uint64(1)..]);
-        if !val.None? && !contents.None? then
-            (Some([val.v] + contents.v), rest2)
-        else
-            (None, [])
+      (None, [])
 }
 
 
 lemma lemma_TupleContents_helper(data:seq<byte>, eltTypes:seq<G>, v:seq<V>, trace:seq<ContentsTraceStep>)
-    requires |data| < 0x1_0000_0000_0000_0000;
-    requires |eltTypes| < 0x1_0000_0000_0000_0000;
-    requires forall elt :: elt in eltTypes ==> ValidGrammar(elt);
-    requires |trace| == |eltTypes| + 1;
-    requires |v| == int(|eltTypes|);
-    requires forall j :: 0 <= j < |trace| ==> |trace[j].data| < 0x1_0000_0000_0000_0000;
-    requires trace[0].data == data;
-    requires forall j :: 0 < j < int(|eltTypes|)+1 ==> 
-                    trace[j].val  == parse_Val(trace[j-1].data, eltTypes[j-1]).0
-                 && trace[j].data == parse_Val(trace[j-1].data, eltTypes[j-1]).1;
-    requires forall j :: 0 < j < |trace| ==> trace[j].val.Some?;
-    requires forall j :: 0 < j < |trace| ==> v[j-1] == trace[j].val.v;
-    //requires v == ExtractValues(trace[1..]);
-    decreases |eltTypes|;
-    ensures  var (v', rest') := parse_Tuple_contents(data, eltTypes);
-             var v_opt := Some(v);
-             v_opt == v' && trace[|trace|-1].data == rest';
+  requires |data| < 0x1_0000_0000_0000_0000
+  requires |eltTypes| < 0x1_0000_0000_0000_0000
+  requires forall elt :: elt in eltTypes ==> ValidGrammar(elt)
+  requires |trace| == |eltTypes| + 1
+  requires |v| == |eltTypes| as int
+  requires forall j :: 0 <= j < |trace| ==> |trace[j].data| < 0x1_0000_0000_0000_0000
+  requires trace[0].data == data
+  requires forall j :: 0 < j < (|eltTypes| as int)+1 ==>
+                 && trace[j].val  == parse_Val(trace[j-1].data, eltTypes[j-1]).0
+                 && trace[j].data == parse_Val(trace[j-1].data, eltTypes[j-1]).1
+  requires forall j :: 0 < j < |trace| ==> trace[j].val.Some?
+  requires forall j :: 0 < j < |trace| ==> v[j-1] == trace[j].val.v
+  //requires v == ExtractValues(trace[1..])
+  decreases |eltTypes|
+  ensures  var (v', rest') := parse_Tuple_contents(data, eltTypes);
+           var v_opt := Some(v);
+           v_opt == v' && trace[|trace|-1].data == rest'
 {
-    reveal_parse_Tuple_contents();
-    if |eltTypes| == 0 {
-    } else {
-        var tuple := parse_Val(data, eltTypes[0]);
-        var val, rest1 := tuple.0, tuple.1;
-        assert trace[1].data == rest1;
-        assert val.Some?;
-        assert trace[1].val == val;
-        lemma_TupleContents_helper(rest1, eltTypes[1..], v[1..], trace[1..]);
-        var tuple'' := parse_Tuple_contents(rest1, eltTypes[1..]);
-        var v'', rest'' := tuple''.0, tuple''.1;
-        var v_opt'' := Some(v[1..]);
-        assert v_opt'' == v'' && trace[1..][|trace[1..]|-1].data == rest'';
+  reveal parse_Tuple_contents();
+  if |eltTypes| == 0 {
+  } else {
+    var tuple := parse_Val(data, eltTypes[0]);
+    var val, rest1 := tuple.0, tuple.1;
+    assert trace[1].data == rest1;
+    assert val.Some?;
+    assert trace[1].val == val;
+    lemma_TupleContents_helper(rest1, eltTypes[1..], v[1..], trace[1..]);
+    var tuple'' := parse_Tuple_contents(rest1, eltTypes[1..]);
+    var v'', rest'' := tuple''.0, tuple''.1;
+    var v_opt'' := Some(v[1..]);
+    assert v_opt'' == v'' && trace[1..][|trace[1..]|-1].data == rest'';
 
-        var tuple' := parse_Tuple_contents(data, eltTypes);
-        var v', rest' := tuple'.0, tuple'.1;
-        calc { 
-            v'; 
-            Some([val.v] + v''.v);
-            Some([val.v] + v[1..]);
-            Some([v[0]] + v[1..]);
-                { assert v == [v[0]] + v[1..]; }
-            Some(v);
-        }
-        assert rest' == rest'';
+    var tuple' := parse_Tuple_contents(data, eltTypes);
+    var v', rest' := tuple'.0, tuple'.1;
+    calc { 
+      v'; 
+      Some([val.v] + v''.v);
+      Some([val.v] + v[1..]);
+      Some([v[0]] + v[1..]);
+        { assert v == [v[0]] + v[1..]; }
+      Some(v);
     }
+    assert rest' == rest'';
+  }
 }
 
 lemma lemma_TupleContents_helper_bailout(data:seq<byte>, eltTypes:seq<G>, trace:seq<ContentsTraceStep>)
-    requires |data| < 0x1_0000_0000_0000_0000;
-    requires |eltTypes| < 0x1_0000_0000_0000_0000;
-    requires forall elt :: elt in eltTypes ==> ValidGrammar(elt);
-    requires 1 < |trace| <= int(|eltTypes|) + 1;
-    requires forall j :: 0 <= j < |trace| ==> |trace[j].data| < 0x1_0000_0000_0000_0000;
-    requires trace[0].data == data;
-    requires forall j :: 0 < j < |trace| ==> 
-                    trace[j].val  == parse_Val(trace[j-1].data, eltTypes[j-1]).0
-                 && trace[j].data == parse_Val(trace[j-1].data, eltTypes[j-1]).1;
-    requires forall j :: 0 < j < |trace| - 1 ==> trace[j].val.Some?;
-    //requires forall j :: 0 < j < |trace| - 1 ==> v[j-1] == trace[j].val.v;
-    requires trace[|trace|-1].val.None?;
-    //requires v == ExtractValues(trace[1..]);
-    decreases |eltTypes|;
-    ensures  var (v', rest') := parse_Tuple_contents(data, eltTypes);
-             v'.None? && rest' == [];
+  requires |data| < 0x1_0000_0000_0000_0000
+  requires |eltTypes| < 0x1_0000_0000_0000_0000
+  requires forall elt :: elt in eltTypes ==> ValidGrammar(elt)
+  requires 1 < |trace| <= (|eltTypes| as int) + 1
+  requires forall j :: 0 <= j < |trace| ==> |trace[j].data| < 0x1_0000_0000_0000_0000
+  requires trace[0].data == data
+  requires forall j :: 0 < j < |trace| ==> 
+                 && trace[j].val  == parse_Val(trace[j-1].data, eltTypes[j-1]).0
+                 && trace[j].data == parse_Val(trace[j-1].data, eltTypes[j-1]).1
+  requires forall j :: 0 < j < |trace| - 1 ==> trace[j].val.Some?
+  //requires forall j :: 0 < j < |trace| - 1 ==> v[j-1] == trace[j].val.v
+  requires trace[|trace|-1].val.None?
+  //requires v == ExtractValues(trace[1..])
+  decreases |eltTypes|
+  ensures  var (v', rest') := parse_Tuple_contents(data, eltTypes);
+           v'.None? && rest' == []
 {
-    reveal_parse_Tuple_contents();
+  reveal parse_Tuple_contents();
     
-    var tuple := parse_Val(data, eltTypes[0]);
-    var val, rest1 := tuple.0, tuple.1;
-    if |trace| == 2 {
-        assert val.None?;
-        var tuple' := parse_Tuple_contents(data, eltTypes);
-        var v', rest' := tuple'.0, tuple'.1;
-        assert v'.None?;
-        assert rest' == [];
-    } else {
-        lemma_TupleContents_helper_bailout(rest1, eltTypes[1..], trace[1..]);
-    }
+  var tuple := parse_Val(data, eltTypes[0]);
+  var val, rest1 := tuple.0, tuple.1;
+  if |trace| == 2 {
+    assert val.None?;
+    var tuple' := parse_Tuple_contents(data, eltTypes);
+    var v', rest' := tuple'.0, tuple'.1;
+    assert v'.None?;
+    assert rest' == [];
+  } else {
+    lemma_TupleContents_helper_bailout(rest1, eltTypes[1..], trace[1..]);
+  }
 }
 
 method{:timeLimitMultiplier 2} ParseTupleContents(data:array<byte>, index:uint64, eltTypes:seq<G>) 
        returns (success:bool, v:seq<V>, rest_index:uint64)
-    requires data != null;
-    requires int(index) <= data.Length;
-    requires data.Length < 0x1_0000_0000_0000_0000;
-    requires |eltTypes| < 0x1_0000_0000_0000_0000;
-    requires forall elt :: elt in eltTypes ==> ValidGrammar(elt);
-    decreases eltTypes, 0;
-    ensures  int(rest_index) <= data.Length;
-    ensures  var (v', rest') := parse_Tuple_contents(data[index..], eltTypes);
-             var v_opt := if success then Some(v) else None();
-             v_opt == v' && data[rest_index..] == rest';
-    ensures  success ==> ValidVal(VTuple(v));
+  requires index as int <= data.Length
+  requires data.Length < 0x1_0000_0000_0000_0000
+  requires |eltTypes| < 0x1_0000_0000_0000_0000
+  requires forall elt :: elt in eltTypes ==> ValidGrammar(elt)
+  decreases eltTypes, 0
+  ensures  rest_index as int <= data.Length
+  ensures  var (v', rest') := parse_Tuple_contents(data[index..], eltTypes);
+           var v_opt := if success then Some(v) else None();
+           v_opt == v' && data[rest_index..] == rest'
+  ensures  success ==> ValidVal(VTuple(v))
 {
-    reveal_parse_Tuple_contents();
-    var vArr := new V[uint64(|eltTypes|)];
-    ghost var g_v := [];
-    success := true;
-    var i:uint64 := 0;
-    var next_val_index:uint64 := index;
-    ghost var trace := [ContentsTraceStep(data[index..], None())];
+  reveal parse_Tuple_contents();
+  var vArr := new V[|eltTypes|];
+  ghost var g_v := [];
+  success := true;
+  var i:int := 0;
+  var next_val_index:uint64 := index;
+  ghost var trace := [ContentsTraceStep(data[index..], None())];
 
-    while i < uint64(|eltTypes|) 
-        invariant 0 <= int(i) <= |eltTypes|;
-        invariant index <= next_val_index <= uint64(data.Length);
-        invariant |trace| == int(i) + 1;
-        invariant |g_v| == int(i);
-        invariant vArr[..i] == g_v;
-        invariant trace[0].data == data[index..];
-        invariant forall j :: 0 <= j < int(i)+1 ==> |trace[j].data| < 0x1_0000_0000_0000_0000;
-        invariant trace[i].data == data[next_val_index..];
-        invariant forall j :: 0 < j <= i ==> trace[j].val.Some?;
-        invariant forall j :: 0 < j <= i ==> g_v[j-1] == trace[j].val.v;
-        invariant forall j :: 0 < j < int(i)+1 ==> 
-            trace[j].val  == parse_Val(trace[j-1].data, eltTypes[j-1]).0
-         && trace[j].data == parse_Val(trace[j-1].data, eltTypes[j-1]).1
-        invariant ValidVal(VTuple(vArr[..i]));
-    {
-        var some1, val, rest1 := ParseVal(data, next_val_index, eltTypes[i]);
-        ghost var step := ContentsTraceStep(data[rest1..], if some1 then Some(val) else None());
-        ghost var old_trace := trace;
-        trace := trace + [step];
-        if !some1 {
-            success := false;
-            rest_index := uint64(data.Length);
-            lemma_TupleContents_helper_bailout(data[index..], eltTypes, trace);
-            return;
-        }
-        g_v := g_v + [val];
-        vArr[i] := val;
-        next_val_index := rest1;
-
-        i := i + 1;
+  while i < |eltTypes|
+    invariant 0 <= i <= |eltTypes|
+    invariant index <= next_val_index <= data.Length as uint64
+    invariant |trace| == i + 1
+    invariant |g_v| == i
+    invariant vArr[..i] == g_v
+    invariant trace[0].data == data[index..]
+    invariant forall j :: 0 <= j < i+1 ==> |trace[j].data| < 0x1_0000_0000_0000_0000
+    invariant trace[i].data == data[next_val_index..]
+    invariant forall j :: 0 < j <= i ==> trace[j].val.Some?
+    invariant forall j :: 0 < j <= i ==> g_v[j-1] == trace[j].val.v
+    invariant forall j :: 0 < j < i+1 ==> 
+                    && trace[j].val  == parse_Val(trace[j-1].data, eltTypes[j-1]).0
+                    && trace[j].data == parse_Val(trace[j-1].data, eltTypes[j-1]).1
+    invariant ValidVal(VTuple(vArr[..i]))
+  {
+    var some1, val, rest1 := ParseVal(data, next_val_index, eltTypes[i]);
+    ghost var step := ContentsTraceStep(data[rest1..], if some1 then Some(val) else None());
+    ghost var old_trace := trace;
+    trace := trace + [step];
+    if !some1 {
+      success := false;
+      rest_index := data.Length as uint64;
+      lemma_TupleContents_helper_bailout(data[index..], eltTypes, trace);
+      return;
     }
+    g_v := g_v + [val];
+    vArr[i] := val;
+    next_val_index := rest1;
 
-    success := true;
-    rest_index := next_val_index;
-    v := vArr[..];               
-    lemma_TupleContents_helper(data[index..], eltTypes, v, trace);
+    i := i + 1;
+  }
+
+  success := true;
+  rest_index := next_val_index;
+  v := vArr[..];               
+  lemma_TupleContents_helper(data[index..], eltTypes, v, trace);
 }
 
 function method parse_Tuple(data:seq<byte>, eltTypes:seq<G>) : (Option<V>, seq<byte>)
-    requires |data| < 0x1_0000_0000_0000_0000;
-    requires |eltTypes| < 0x1_0000_0000_0000_0000;
-    requires forall elt :: elt in eltTypes ==> ValidGrammar(elt);
-    decreases eltTypes, 1;
-    ensures var (opt_val, rest) := parse_Tuple(data, eltTypes);
-            |rest| <= |data| && (opt_val.Some? ==> ValInGrammar(opt_val.v, GTuple(eltTypes)));
+  requires |data| < 0x1_0000_0000_0000_0000
+  requires |eltTypes| < 0x1_0000_0000_0000_0000
+  requires forall elt :: elt in eltTypes ==> ValidGrammar(elt)
+  decreases eltTypes, 1
+  ensures var (opt_val, rest) := parse_Tuple(data, eltTypes);
+          |rest| <= |data| && (opt_val.Some? ==> ValInGrammar(opt_val.v, GTuple(eltTypes)))
 {
-    var (contents, rest) := parse_Tuple_contents(data, eltTypes);
-    if !contents.None? then
-        (Some(VTuple(contents.v)), rest)
-    else
-        (None, [])
+  var (contents, rest) := parse_Tuple_contents(data, eltTypes);
+  if !contents.None? then
+    (Some(VTuple(contents.v)), rest)
+  else
+    (None, [])
 }
 
 
 method ParseTuple(data:array<byte>, index:uint64, eltTypes:seq<G>) returns (success:bool, v:V, rest_index:uint64)
-    requires data != null;
-    requires int(index) <= data.Length;
-    requires data.Length < 0x1_0000_0000_0000_0000;
-    requires |eltTypes| < 0x1_0000_0000_0000_0000;
-    requires forall elt :: elt in eltTypes ==> ValidGrammar(elt);
-    decreases eltTypes, 1;
-    ensures  int(rest_index) <= data.Length;
-    ensures  var (v', rest') := parse_Tuple(data[index..], eltTypes);
-             var v_opt := if success then Some(v) else None();
-             v_opt == v' && data[rest_index..] == rest';
-    ensures  success ==> ValidVal(v);
+  requires index as int <= data.Length
+  requires data.Length < 0x1_0000_0000_0000_0000
+  requires |eltTypes| < 0x1_0000_0000_0000_0000
+  requires forall elt :: elt in eltTypes ==> ValidGrammar(elt)
+  decreases eltTypes, 1
+  ensures  rest_index as int <= data.Length
+  ensures  var (v', rest') := parse_Tuple(data[index..], eltTypes);
+           var v_opt := if success then Some(v) else None();
+           v_opt == v' && data[rest_index..] == rest'
+  ensures  success ==> ValidVal(v);
 {
-    var some, contents, rest := ParseTupleContents(data, index, eltTypes);
-    if some {
-        success := true;
-        v := VTuple(contents);
-        rest_index := rest;
-    } else {
-        success := false;
-        rest_index := uint64(data.Length);
-    }
+  var some, contents, rest := ParseTupleContents(data, index, eltTypes);
+  if some {
+    success := true;
+    v := VTuple(contents);
+    rest_index := rest;
+  } else {
+    success := false;
+    rest_index := data.Length as uint64;
+  }
 }
 
 function method parse_ByteArray(data:seq<byte>) : (Option<V>, seq<byte>)
-    requires |data| < 0x1_0000_0000_0000_0000;
+  requires |data| < 0x1_0000_0000_0000_0000
 {
-    var (len, rest) := parse_Uint64(data);
-    if !len.None? && len.v.u <= uint64(|rest|) then
-        (Some(VByteArray(rest[uint64(0)..len.v.u])), rest[len.v.u..])
-    else
-        (None, [])
+  var (len, rest) := parse_Uint64(data);
+  if !len.None? && len.v.u <= |rest| as uint64 then
+    (Some(VByteArray(rest[0..len.v.u])), rest[len.v.u..])
+  else
+    (None, [])
 }
 
 method ParseByteArray(data:array<byte>, index:uint64) returns (success:bool, v:V, rest_index:uint64)
-    requires data != null;
-    requires int(index) <= data.Length;
-    requires data.Length < 0x1_0000_0000_0000_0000;
-    ensures  int(rest_index) <= data.Length;
-    ensures  var (v', rest') := parse_ByteArray(data[index..]);
-             var v_opt := if success then Some(v) else None();
-             v_opt == v' && data[rest_index..] == rest';
+  requires index as int <= data.Length
+  requires data.Length < 0x1_0000_0000_0000_0000
+  ensures  rest_index as int <= data.Length
+  ensures  var (v', rest') := parse_ByteArray(data[index..]);
+           var v_opt := if success then Some(v) else None();
+           v_opt == v' && data[rest_index..] == rest'
 {
-    var some, len, rest := ParseUint64(data, index);
-    if some && len.u <= uint64(data.Length) - rest {
-        var rest_seq := data[rest..];
-        assert len.u <= uint64(|rest_seq|);
-        calc {
-            rest_seq[0..len.u];
-            data[rest..rest + len.u];
-        }
-        success := true;
-        v := VByteArray(data[rest..rest + len.u]);
-        rest_index := rest + len.u;
-    } else {
-        success := false;
-        rest_index := uint64(data.Length);
+  var some, len, rest := ParseUint64(data, index);
+  if some && len.u <= data.Length as uint64 - rest {
+    var rest_seq := data[rest..];
+    assert len.u <= |rest_seq| as uint64;
+    calc {
+      rest_seq[0..len.u];
+      data[rest..rest + len.u];
     }
+    success := true;
+    v := VByteArray(data[rest..rest + len.u]);
+    rest_index := rest + len.u;
+  } else {
+    success := false;
+    rest_index := data.Length as uint64;
+  }
 }
 
 function method parse_Case(data:seq<byte>, cases:seq<G>) : (Option<V>, seq<byte>)
-    requires |data| < 0x1_0000_0000_0000_0000;
-    requires |cases| < 0x1_0000_0000_0000_0000;
-    requires forall elt :: elt in cases ==> ValidGrammar(elt);
-    decreases cases;
-    ensures var (opt_val, rest) := parse_Case(data, cases);
-            |rest| <= |data| && (opt_val.Some? ==> ValInGrammar(opt_val.v, GTaggedUnion(cases)));
+  requires |data| < 0x1_0000_0000_0000_0000
+  requires |cases| < 0x1_0000_0000_0000_0000
+  requires forall elt :: elt in cases ==> ValidGrammar(elt)
+  decreases cases
+  ensures var (opt_val, rest) := parse_Case(data, cases);
+          |rest| <= |data| && (opt_val.Some? ==> ValInGrammar(opt_val.v, GTaggedUnion(cases)))
 {
-    var (caseID, rest1) := parse_Uint64(data);
+  var (caseID, rest1) := parse_Uint64(data);
 
-    if !caseID.None? && caseID.v.u < uint64(|cases|) then
-        var (val, rest2) := parse_Val(rest1, cases[caseID.v.u]);
-        if !val.None? then
-            (Some(VCase(caseID.v.u, val.v)), rest2)
-        else
-            (None, [])
+  if !caseID.None? && caseID.v.u < |cases| as uint64 then
+    var (val, rest2) := parse_Val(rest1, cases[caseID.v.u]);
+    if !val.None? then
+      (Some(VCase(caseID.v.u, val.v)), rest2)
     else
-        (None, [])
+      (None, [])
+  else
+    (None, [])
 }
 
 method ParseCase(data:array<byte>, index:uint64, cases:seq<G>) returns (success:bool, v:V, rest_index:uint64)
-    requires data != null;
-    requires int(index) <= data.Length;
-    requires data.Length < 0x1_0000_0000_0000_0000;
-    requires |cases| < 0x1_0000_0000_0000_0000;
-    requires forall elt :: elt in cases ==> ValidGrammar(elt);
-    decreases cases;
-    ensures  int(rest_index) <= data.Length;
-    ensures  var (v', rest') := parse_Case(data[index..], cases);
-             var v_opt := if success then Some(v) else None();
-             v_opt == v' && data[rest_index..] == rest';
-    ensures  success ==> ValidVal(v);
+  requires index as int <= data.Length
+  requires data.Length < 0x1_0000_0000_0000_0000
+  requires |cases| < 0x1_0000_0000_0000_0000
+  requires forall elt :: elt in cases ==> ValidGrammar(elt)
+  decreases cases
+  ensures  rest_index as int <= data.Length
+  ensures  var (v', rest') := parse_Case(data[index..], cases);
+           var v_opt := if success then Some(v) else None();
+           v_opt == v' && data[rest_index..] == rest'
+  ensures  success ==> ValidVal(v)
 {
-    var some1, caseID, rest1 := ParseUint64(data, index);
+  var some1, caseID, rest1 := ParseUint64(data, index);
 
-    if some1 && caseID.u < uint64(|cases|) {
-        var some2, val, rest2 := ParseVal(data, rest1, cases[caseID.u]);
-        if some2 {
-            success := true;
-            v := VCase(caseID.u, val);
-            rest_index := rest2;
-        } else {
-            success := false;
-            rest_index := uint64(data.Length);
-        }
+  if some1 && caseID.u < |cases| as uint64 {
+    var some2, val, rest2 := ParseVal(data, rest1, cases[caseID.u]);
+    if some2 {
+      success := true;
+      v := VCase(caseID.u, val);
+      rest_index := rest2;
     } else {
-        success := false;
-        rest_index := uint64(data.Length);
+      success := false;
+      rest_index := data.Length as uint64;
     }
+  } else {
+    success := false;
+    rest_index := data.Length as uint64;
+  }
 }
 
 function method {:opaque} parse_Val(data:seq<byte>, grammar:G) : (Option<V>, seq<byte>)
-    requires |data| < 0x1_0000_0000_0000_0000;
-    requires ValidGrammar(grammar);
-    decreases grammar, 0;
-    ensures  var (val, rest) := parse_Val(data, grammar);
-             |rest| <= |data| && (!val.None? ==> ValInGrammar(val.v, grammar));
+  requires |data| < 0x1_0000_0000_0000_0000
+  requires ValidGrammar(grammar)
+  decreases grammar, 0
+  ensures  var (val, rest) := parse_Val(data, grammar);
+           |rest| <= |data| && (!val.None? ==> ValInGrammar(val.v, grammar))
 {
-    match grammar
-        case GUint64             => parse_Uint64(data)
-        case GArray(elt)         => parse_Array(data, elt)
-        case GTuple(t)           => parse_Tuple(data, t)
-        case GByteArray          => parse_ByteArray(data)
-        case GTaggedUnion(cases) => parse_Case(data, cases)
+  match grammar
+    case GUint64             => parse_Uint64(data)
+    case GArray(elt)         => parse_Array(data, elt)
+    case GTuple(t)           => parse_Tuple(data, t)
+    case GByteArray          => parse_ByteArray(data)
+    case GTaggedUnion(cases) => parse_Case(data, cases)
 }
 
 method ParseVal(data:array<byte>, index:uint64, grammar:G) returns (success:bool, v:V, rest_index:uint64)
-    requires data != null;
-    requires int(index) <= data.Length;
-    requires data.Length < 0x1_0000_0000_0000_0000;
-    requires ValidGrammar(grammar);
-    decreases grammar, 0;
-    ensures  int(rest_index) <= data.Length;
-    ensures  var (v', rest') := parse_Val(data[index..], grammar);
-             var v_opt := if success then Some(v) else None();
-             v_opt == v' && data[rest_index..] == rest';
-    ensures  success ==> ValidVal(v);
+  requires index as int <= data.Length
+  requires data.Length < 0x1_0000_0000_0000_0000
+  requires ValidGrammar(grammar)
+  decreases grammar, 0
+  ensures  rest_index as int <= data.Length
+  ensures  var (v', rest') := parse_Val(data[index..], grammar);
+           var v_opt := if success then Some(v) else None();
+           v_opt == v' && data[rest_index..] == rest'
+  ensures  success ==> ValidVal(v);
 {
-    reveal_parse_Val();
+  reveal parse_Val();
 
-    match grammar {
-        case GUint64             => success, v, rest_index := ParseUint64(data, index);
-        case GArray(elt)         => success, v, rest_index := ParseArray(data, index, elt);
-        case GTuple(t)           => success, v, rest_index := ParseTuple(data, index, t);
-        case GByteArray          => success, v, rest_index := ParseByteArray(data, index);
-        case GTaggedUnion(cases) => success, v, rest_index := ParseCase(data, index, cases);
-    }
+  match grammar {
+    case GUint64             => success, v, rest_index := ParseUint64(data, index);
+    case GArray(elt)         => success, v, rest_index := ParseArray(data, index, elt);
+    case GTuple(t)           => success, v, rest_index := ParseTuple(data, index, t);
+    case GByteArray          => success, v, rest_index := ParseByteArray(data, index);
+    case GTaggedUnion(cases) => success, v, rest_index := ParseCase(data, index, cases);
+  }
 }
 
 predicate Demarshallable(data:seq<byte>, grammar:G)
 {
-       |data| < 0x1_0000_0000_0000_0000
-    && ValidGrammar(grammar)
-    && !parse_Val(data, grammar).0.None?
-    && ValidVal(parse_Val(data, grammar).0.v)
-    && parse_Val(data, grammar).1 == []
+  && |data| < 0x1_0000_0000_0000_0000
+  && ValidGrammar(grammar)
+  && !parse_Val(data, grammar).0.None?
+  && ValidVal(parse_Val(data, grammar).0.v)
+  && parse_Val(data, grammar).1 == []
 }
 
 function DemarshallFunc(data:seq<byte>, grammar:G) : V
-    requires Demarshallable(data, grammar);
-    decreases grammar, 0;
-    ensures  var (val, rest) := parse_Val(data, grammar);
-             !val.None? && ValInGrammar(val.v, grammar);
+  requires Demarshallable(data, grammar)
+  decreases grammar, 0
+  ensures  var (val, rest) := parse_Val(data, grammar);
+           !val.None? && ValInGrammar(val.v, grammar)
 {
-    parse_Val(data, grammar).0.v
+  parse_Val(data, grammar).0.v
 }
 
 method Demarshall(data:array<byte>, grammar:G) returns (success:bool, v:V)
-    requires data != null;
-    requires data.Length < 0x1_0000_0000_0000_0000;
-    requires ValidGrammar(grammar);
-    ensures  success == Demarshallable(data[..], grammar);
-    ensures  success ==> v == DemarshallFunc(data[..], grammar);
+  requires data.Length < 0x1_0000_0000_0000_0000
+  requires ValidGrammar(grammar)
+  ensures  success == Demarshallable(data[..], grammar)
+  ensures  success ==> v == DemarshallFunc(data[..], grammar)
 {
-    var rest:uint64;
-    success, v, rest := ParseVal(data, 0, grammar);
-    if success && rest == uint64(data.Length) {
-        assert v == parse_Val(data[..], grammar).0.v;
-        assert Demarshallable(data[..], grammar);
-        assert v == DemarshallFunc(data[..], grammar);
-    } else {
-        success := false;
-        assert !Demarshallable(data[..], grammar);
-    }
+  var rest:uint64;
+  success, v, rest := ParseVal(data, 0, grammar);
+  if success && rest == data.Length as uint64 {
+    assert v == parse_Val(data[..], grammar).0.v;
+    assert Demarshallable(data[..], grammar);
+    assert v == DemarshallFunc(data[..], grammar);
+  } else {
+    success := false;
+    assert !Demarshallable(data[..], grammar);
+  }
 }
 
 
 lemma lemma_parse_Val_view_ByteArray(data:seq<byte>, v:V, grammar:G, index:int)
-    requires |data| < 0x1_0000_0000_0000_0000;
-    requires ValInGrammar(v, grammar);
-    requires ValidGrammar(grammar);
-    requires grammar.GByteArray?;
-    requires 0 <= index <= |data|;
-    requires 0 <= index + SizeOfV(v) <= |data|;
-    ensures  forall bound :: Trigger(bound) ==> (index+SizeOfV(v) <= bound <= |data| ==>
-             ((parse_ByteArray(data[index..bound]).0 == Some(v)) <==> (parse_ByteArray(data[index..index+SizeOfV(v)]).0 == Some(v))));
-    ensures  forall bound :: index+SizeOfV(v) <= bound <= |data| ==>
-             parse_ByteArray(data[index..bound]).0 == Some(v) ==> parse_ByteArray(data[index..bound]).1 == data[index+SizeOfV(v)..bound];
+  requires |data| < 0x1_0000_0000_0000_0000
+  requires ValInGrammar(v, grammar)
+  requires ValidGrammar(grammar)
+  requires grammar.GByteArray?
+  requires 0 <= index <= |data|
+  requires 0 <= index + SizeOfV(v) <= |data|
+  ensures  forall bound :: Trigger(bound) ==> (index+SizeOfV(v) <= bound <= |data| ==>
+             ((parse_ByteArray(data[index..bound]).0 == Some(v)) <==> (parse_ByteArray(data[index..index+SizeOfV(v)]).0 == Some(v))))
+  ensures  forall bound :: index+SizeOfV(v) <= bound <= |data| ==>
+             parse_ByteArray(data[index..bound]).0 == Some(v) ==> parse_ByteArray(data[index..bound]).1 == data[index+SizeOfV(v)..bound]
 {
-    forall bound {:trigger Trigger(bound)} | Trigger(bound)
-        ensures index+SizeOfV(v) <= bound <= |data| ==> ((parse_ByteArray(data[index..bound]).0 == Some(v)) <==> (parse_ByteArray(data[index..index+SizeOfV(v)]).0 == Some(v)));
-    {
-        if index+SizeOfV(v) <= bound <= |data| {
-            var narrow_tuple := parse_ByteArray(data[index..index+SizeOfV(v)]);
-            var bound_tuple := parse_ByteArray(data[index..bound]);
-            var narrow_len_tuple := parse_Uint64(data[index..index+SizeOfV(v)]);
-            var bound_len_tuple := parse_Uint64(data[index..bound]);
-            assert narrow_len_tuple.0 == bound_len_tuple.0;
+  forall bound {:trigger Trigger(bound)} | Trigger(bound)
+    ensures index+SizeOfV(v) <= bound <= |data| ==>
+              ((parse_ByteArray(data[index..bound]).0 == Some(v)) <==> (parse_ByteArray(data[index..index+SizeOfV(v)]).0 == Some(v)))
+  {
+    if index+SizeOfV(v) <= bound <= |data| {
+      var narrow_tuple := parse_ByteArray(data[index..index+SizeOfV(v)]);
+      var bound_tuple := parse_ByteArray(data[index..bound]);
+      var narrow_len_tuple := parse_Uint64(data[index..index+SizeOfV(v)]);
+      var bound_len_tuple := parse_Uint64(data[index..bound]);
+      assert narrow_len_tuple.0 == bound_len_tuple.0;
 
-            if bound_tuple.0 == Some(v) {
-                assert bound_len_tuple.1[0..bound_len_tuple.0.v.u] == narrow_len_tuple.1[0..bound_len_tuple.0.v.u];     // OBSERVE
-            }
+      if bound_tuple.0 == Some(v) {
+        assert bound_len_tuple.1[0..bound_len_tuple.0.v.u] == narrow_len_tuple.1[0..bound_len_tuple.0.v.u];     // OBSERVE
+      }
 
-            if narrow_tuple.0 == Some(v) {
-                assert bound_len_tuple.1[0..bound_len_tuple.0.v.u] == narrow_len_tuple.1[0..bound_len_tuple.0.v.u];       // OBSERVE
-            }
-            assert ((parse_ByteArray(data[index..bound]).0 == Some(v)) <==> (parse_ByteArray(data[index..index+SizeOfV(v)]).0 == Some(v)));
-        }
-        assert index+SizeOfV(v) <= bound <= |data| ==> ((parse_ByteArray(data[index..bound]).0 == Some(v)) <==> (parse_ByteArray(data[index..index+SizeOfV(v)]).0 == Some(v)));
+      if narrow_tuple.0 == Some(v) {
+        assert bound_len_tuple.1[0..bound_len_tuple.0.v.u] == narrow_len_tuple.1[0..bound_len_tuple.0.v.u];       // OBSERVE
+      }
+      assert ((parse_ByteArray(data[index..bound]).0 == Some(v)) <==> (parse_ByteArray(data[index..index+SizeOfV(v)]).0 == Some(v)));
     }
-    assert forall bound :: Trigger(bound) ==> (index+SizeOfV(v) <= bound <= |data| ==>
-             ((parse_ByteArray(data[index..bound]).0 == Some(v)) <==> (parse_ByteArray(data[index..index+SizeOfV(v)]).0 == Some(v))));
-    assert forall bound :: index+SizeOfV(v) <= bound <= |data| ==>
-             parse_ByteArray(data[index..bound]).0 == Some(v) ==> parse_ByteArray(data[index..bound]).1 == data[index+SizeOfV(v)..bound];
+    assert index+SizeOfV(v) <= bound <= |data| ==> ((parse_ByteArray(data[index..bound]).0 == Some(v)) <==> (parse_ByteArray(data[index..index+SizeOfV(v)]).0 == Some(v)));
+  }
+  assert forall bound :: Trigger(bound) ==> (index+SizeOfV(v) <= bound <= |data| ==>
+           ((parse_ByteArray(data[index..bound]).0 == Some(v)) <==> (parse_ByteArray(data[index..index+SizeOfV(v)]).0 == Some(v))));
+  assert forall bound :: index+SizeOfV(v) <= bound <= |data| ==>
+           parse_ByteArray(data[index..bound]).0 == Some(v) ==> parse_ByteArray(data[index..bound]).1 == data[index+SizeOfV(v)..bound];
 }
 
 lemma lemma_SeqSum_prefix(s:seq<V>, v:V)
-    ensures SeqSum(s + [v]) == SeqSum(s) + SizeOfV(v);
+  ensures SeqSum(s + [v]) == SeqSum(s) + SizeOfV(v)
 {
-    reveal_SeqSum();
-    if |s| == 0 {
-    } else {
-        calc {
-            SeqSum(s + [v]);
-                { assert (s + [v])[0] == s[0];  
-                  assert (s + [v])[1..] == s[1..]+[v]; }
-            SizeOfV(s[0]) + SeqSum(s[1..] + [v]);
-                { lemma_SeqSum_prefix(s[1..], v); }
-            SizeOfV(s[0]) + SeqSum(s[1..]) + SizeOfV(v);
-            SeqSum(s) + SizeOfV(v);
-        }
+  reveal SeqSum();
+  if |s| == 0 {
+  } else {
+    calc {
+      SeqSum(s + [v]);
+        { assert (s + [v])[0] == s[0];  
+          assert (s + [v])[1..] == s[1..]+[v]; }
+      SizeOfV(s[0]) + SeqSum(s[1..] + [v]);
+        { lemma_SeqSum_prefix(s[1..], v); }
+      SizeOfV(s[0]) + SeqSum(s[1..]) + SizeOfV(v);
+      SeqSum(s) + SizeOfV(v);
     }
+  }
 }
 
 lemma lemma_SeqSum_bound(s:seq<V>, bound:int)
-    requires SeqSum(s) < bound;
-    ensures  forall v :: v in s ==> SizeOfV(v) < bound;
+  requires SeqSum(s) < bound
+  ensures  forall v :: v in s ==> SizeOfV(v) < bound
 {
-    reveal_SeqSum();
-    if |s| == 0 {
-    } else {
-        assert SizeOfV(s[0]) + SeqSum(s[1..]) < bound;
-        assert SizeOfV(s[0]) < bound;
-        lemma_SeqSum_bound(s[1..], bound);
-    }
+  reveal SeqSum();
+  if |s| == 0 {
+  } else {
+    assert SizeOfV(s[0]) + SeqSum(s[1..]) < bound;
+    assert SizeOfV(s[0]) < bound;
+    lemma_SeqSum_bound(s[1..], bound);
+  }
 }
 
 lemma lemma_SeqSum_bound_prefix(s:seq<V>, prefix:seq<V>, index:int)
-    requires 0 <= index <= |s|;
-    requires prefix == s[..index];
-    ensures  SeqSum(prefix) <= SeqSum(s);
+  requires 0 <= index <= |s|
+  requires prefix == s[..index]
+  ensures  SeqSum(prefix) <= SeqSum(s)
 {
-    reveal_SeqSum();
-    if |prefix| == 0 {
-    } else {
-        lemma_SeqSum_bound_prefix(s[1..], prefix[1..], index - 1);
-    }
+  reveal SeqSum();
+  if |prefix| == 0 {
+  } else {
+    lemma_SeqSum_bound_prefix(s[1..], prefix[1..], index - 1);
+  }
 }
 
 lemma lemma_parse_Array_contents_len(data:seq<byte>, eltType:G, len:uint64)
-    requires |data| < 0x1_0000_0000_0000_0000;
-    requires ValidGrammar(eltType);
-    requires len >= 0;
-    requires !parse_Array_contents(data, eltType, len).0.None?;
-    decreases len;
-    ensures  int(len) == |parse_Array_contents(data, eltType, len).0.v|;
+  requires |data| < 0x1_0000_0000_0000_0000
+  requires ValidGrammar(eltType)
+  requires len >= 0
+  requires !parse_Array_contents(data, eltType, len).0.None?
+  decreases len
+  ensures  len as int == |parse_Array_contents(data, eltType, len).0.v|
 {
-    reveal_parse_Array_contents();
-    if len == 0 {
-    } else {
-       var tuple1 := parse_Val(data, eltType);
-       var val   := tuple1.0;
-       var rest1 := tuple1.1;
-       var tuple2 := parse_Array_contents(rest1, eltType, len - 1);
-       var others := tuple2.0;
-       var rest2  := tuple2.1;
-       assert !val.None? && !others.None?;
-       lemma_parse_Array_contents_len(rest1, eltType, len - 1);
-    }
+  reveal parse_Array_contents();
+  if len == 0 {
+  } else {
+    var tuple1 := parse_Val(data, eltType);
+    var val   := tuple1.0;
+    var rest1 := tuple1.1;
+    var tuple2 := parse_Array_contents(rest1, eltType, len - 1);
+    var others := tuple2.0;
+    var rest2  := tuple2.1;
+    assert !val.None? && !others.None?;
+    lemma_parse_Array_contents_len(rest1, eltType, len - 1);
+  }
 }
 
 lemma lemma_parse_Val_view_Array_contents(data:seq<byte>, vs:seq<V>, grammar:G, index:int, bound:int, len:uint64)
-    requires |data| < 0x1_0000_0000_0000_0000;
-    requires forall v :: v in vs ==> ValInGrammar(v, grammar);
-    requires ValidGrammar(grammar);
-    requires int(len) == |vs|;
-    requires 0 <= index <= |data|;
-    requires 0 <= index + SeqSum(vs) <= |data|;
-    requires index+SeqSum(vs) <= bound <= |data|;
-    decreases grammar, 1, len;
-    //decreases |vs|;
-    ensures  (parse_Array_contents(data[index..bound], grammar, len).0 == Some(vs)) <==> (parse_Array_contents(data[index..index+SeqSum(vs)], grammar, len).0 == Some(vs));
-    ensures  parse_Array_contents(data[index..bound], grammar, len).0 == Some(vs) ==> parse_Array_contents(data[index..bound], grammar, len).1 == data[index+SeqSum(vs)..bound];
+  requires |data| < 0x1_0000_0000_0000_0000
+  requires forall v :: v in vs ==> ValInGrammar(v, grammar)
+  requires ValidGrammar(grammar)
+  requires len as int == |vs|
+  requires 0 <= index <= |data|
+  requires 0 <= index + SeqSum(vs) <= |data|
+  requires index+SeqSum(vs) <= bound <= |data|
+  decreases grammar, 1, len
+  //decreases |vs|
+  ensures  (parse_Array_contents(data[index..bound], grammar, len).0 == Some(vs)) <==> (parse_Array_contents(data[index..index+SeqSum(vs)], grammar, len).0 == Some(vs))
+  ensures  parse_Array_contents(data[index..bound], grammar, len).0 == Some(vs) ==> parse_Array_contents(data[index..bound], grammar, len).1 == data[index+SeqSum(vs)..bound]
 {
-    reveal_parse_Array_contents();
-    if len == 0 {
-        reveal_SeqSum();
+  reveal parse_Array_contents();
+  if len == 0 {
+    reveal SeqSum();
+  } else {
+    var narrow_tuple := parse_Array_contents(data[index..index+SeqSum(vs)], grammar, len);
+    var bound_tuple := parse_Array_contents(data[index..bound], grammar, len);
+    var narrow_val_tuple := parse_Val(data[index..index+SeqSum(vs)], grammar);
+    var bound_val_tuple := parse_Val(data[index..bound], grammar);
+    var narrow_contents_tuple := parse_Array_contents(narrow_val_tuple.1, grammar, len - 1);
+    var bound_contents_tuple := parse_Array_contents(bound_val_tuple.1, grammar, len - 1);
+
+
+    if narrow_tuple.0 == Some(vs) {
+      assert !narrow_val_tuple.0.None? && !narrow_contents_tuple.0.None?;
+      calc {
+        index + SeqSum(vs) <= |data|;
+        SeqSum(vs) <= |data| - index;
+        SeqSum(vs) < |data| - index + 1;
+      }
+      lemma_SeqSum_bound(vs, |data| - index + 1);
+      lemma_parse_Val_view(data, vs[0], grammar, index);
+
+      lemma_SeqSum_bound(vs, SeqSum(vs) + 1);
+      assert index+SizeOfV(vs[0]) <= bound <= |data|;
+      assert (parse_Val(data[index..index+SeqSum(vs)], grammar).0 == Some(vs[0])) <==> (parse_Val(data[index..index+SizeOfV(vs[0])], grammar).0 == Some(vs[0]));
+      lemma_SeqSum_bound(vs, bound - index + 1);
+      assert index+SizeOfV(vs[0]) <= bound <= |data|;     // OBSERVE (trigger on forall?)
+      assert (parse_Val(data[index..bound], grammar).0 == Some(vs[0])) <==> (parse_Val(data[index..index+SizeOfV(vs[0])], grammar).0 == Some(vs[0]));
+      assert narrow_val_tuple.0.v == vs[0] == bound_val_tuple.0.v;
+
+      var new_index := index + SizeOfV(narrow_val_tuple.0.v);
+      calc {
+        SizeOfV(narrow_val_tuple.0.v) + SeqSum(vs[1..]);
+          { reveal SeqSum(); }
+        SeqSum(vs);
+      }
+      assert new_index+SeqSum(vs[1..]) <= bound;
+
+      lemma_parse_Val_view_Array_contents(data, vs[1..], grammar, new_index, bound, len - 1);
+
+      assert (parse_Array_contents(data[new_index..bound], grammar, len - 1).0 == Some(vs[1..])) <==> (parse_Array_contents(data[new_index..new_index+SeqSum(vs[1..])], grammar, len - 1).0 == Some(vs[1..]));
+      assert data[new_index..new_index+SeqSum(vs[1..])] == narrow_val_tuple.1;
+      assert data[new_index..bound] == bound_val_tuple.1;
+
+      assert bound_tuple.0 == Some([vs[0]] + vs[1..]) == Some(vs);
+    } else if bound_tuple.0 == Some(vs) {
+      assert !bound_val_tuple.0.None? && !bound_contents_tuple.0.None?;
+
+      lemma_SeqSum_bound(vs, |data| - index + 1);
+      lemma_parse_Val_view(data, vs[0], grammar, index);
+      // This is exactly the ensures of the lemma above
+      assert forall bound' :: index+SizeOfV(vs[0]) <= bound' <= |data| ==>
+               ((parse_Val(data[index..bound'], grammar).0 == Some(vs[0])) <==> (parse_Val(data[index..index+SizeOfV(vs[0])], grammar).0 == Some(vs[0])));
+
+      lemma_SeqSum_bound(vs, bound - index + 1);
+      lemma_SeqSum_bound(vs, SeqSum(vs) + 1);
+      assert index+SizeOfV(vs[0]) <= index+SeqSum(vs) <= |data|;
+      assert (parse_Val(data[index..index+SeqSum(vs)], grammar).0 == Some(vs[0])) <==> (parse_Val(data[index..index+SizeOfV(vs[0])], grammar).0 == Some(vs[0]));
+      assert (parse_Val(data[index..bound], grammar).0 == Some(vs[0])) <==> (parse_Val(data[index..index+SizeOfV(vs[0])], grammar).0 == Some(vs[0]));
+      assert narrow_val_tuple.0.v == vs[0] == bound_val_tuple.0.v;
+
+      var new_index := index + SizeOfV(narrow_val_tuple.0.v);
+      calc {
+        SizeOfV(narrow_val_tuple.0.v) + SeqSum(vs[1..]);
+          { reveal SeqSum(); }
+        SeqSum(vs);
+      }
+      assert new_index+SeqSum(vs[1..]) <= bound;
+
+      lemma_parse_Val_view_Array_contents(data, vs[1..], grammar, new_index, bound, len - 1);
+
+      assert (parse_Array_contents(data[new_index..bound], grammar, len - 1).0 == Some(vs[1..])) <==> (parse_Array_contents(data[new_index..new_index+SeqSum(vs[1..])], grammar, len - 1).0 == Some(vs[1..]));
+      assert data[new_index..new_index+SeqSum(vs[1..])] == narrow_val_tuple.1;
+      assert data[new_index..bound] == bound_val_tuple.1;
+
+      assert narrow_tuple.0 == Some([vs[0]] + vs[1..]) == Some(vs);
     } else {
-        var narrow_tuple := parse_Array_contents(data[index..index+SeqSum(vs)], grammar, len);
-        var bound_tuple := parse_Array_contents(data[index..bound], grammar, len);
-        var narrow_val_tuple := parse_Val(data[index..index+SeqSum(vs)], grammar);
-        var bound_val_tuple := parse_Val(data[index..bound], grammar);
-        var narrow_contents_tuple := parse_Array_contents(narrow_val_tuple.1, grammar, len - 1);
-        var bound_contents_tuple := parse_Array_contents(bound_val_tuple.1, grammar, len - 1);
-
-
-        if narrow_tuple.0 == Some(vs) {
-            assert !narrow_val_tuple.0.None? && !narrow_contents_tuple.0.None?;
-            calc {
-                index + SeqSum(vs) <= |data|;
-                SeqSum(vs) <= |data| - index;
-                SeqSum(vs) < |data| - index + 1;
-            }
-            lemma_SeqSum_bound(vs, |data| - index + 1);
-            lemma_parse_Val_view(data, vs[0], grammar, index);
-
-            lemma_SeqSum_bound(vs, SeqSum(vs) + 1);
-            assert index+SizeOfV(vs[0]) <= bound <= |data|;
-            assert (parse_Val(data[index..index+SeqSum(vs)], grammar).0 == Some(vs[0])) <==> (parse_Val(data[index..index+SizeOfV(vs[0])], grammar).0 == Some(vs[0]));
-            lemma_SeqSum_bound(vs, bound - index + 1);
-            assert index+SizeOfV(vs[0]) <= bound <= |data|;     // OBSERVE (trigger on forall?)
-            assert (parse_Val(data[index..bound], grammar).0 == Some(vs[0])) <==> (parse_Val(data[index..index+SizeOfV(vs[0])], grammar).0 == Some(vs[0]));
-            assert narrow_val_tuple.0.v == vs[0] == bound_val_tuple.0.v;
-
-            var new_index := index + SizeOfV(narrow_val_tuple.0.v);
-            calc {
-                SizeOfV(narrow_val_tuple.0.v) + SeqSum(vs[1..]);
-                    { reveal_SeqSum(); }
-                SeqSum(vs);
-            }
-            assert new_index+SeqSum(vs[1..]) <= bound;
-
-            lemma_parse_Val_view_Array_contents(data, vs[1..], grammar, new_index, bound, len - 1);
-
-            assert (parse_Array_contents(data[new_index..bound], grammar, len - 1).0 == Some(vs[1..])) <==> (parse_Array_contents(data[new_index..new_index+SeqSum(vs[1..])], grammar, len - 1).0 == Some(vs[1..]));
-            assert data[new_index..new_index+SeqSum(vs[1..])] == narrow_val_tuple.1;
-            assert data[new_index..bound] == bound_val_tuple.1;
-
-            assert bound_tuple.0 == Some([vs[0]] + vs[1..]) == Some(vs);
-        } else if bound_tuple.0 == Some(vs) {
-            assert !bound_val_tuple.0.None? && !bound_contents_tuple.0.None?;
-
-            lemma_SeqSum_bound(vs, |data| - index + 1);
-            lemma_parse_Val_view(data, vs[0], grammar, index);
-            // This is exactly the ensures of the lemma above
-            assert forall bound' :: index+SizeOfV(vs[0]) <= bound' <= |data| ==>
-                   ((parse_Val(data[index..bound'], grammar).0 == Some(vs[0])) <==> (parse_Val(data[index..index+SizeOfV(vs[0])], grammar).0 == Some(vs[0])));
-
-            lemma_SeqSum_bound(vs, bound - index + 1);
-            lemma_SeqSum_bound(vs, SeqSum(vs) + 1);
-            assert index+SizeOfV(vs[0]) <= index+SeqSum(vs) <= |data|;
-            assert (parse_Val(data[index..index+SeqSum(vs)], grammar).0 == Some(vs[0])) <==> (parse_Val(data[index..index+SizeOfV(vs[0])], grammar).0 == Some(vs[0]));
-            assert (parse_Val(data[index..bound], grammar).0 == Some(vs[0])) <==> (parse_Val(data[index..index+SizeOfV(vs[0])], grammar).0 == Some(vs[0]));
-            assert narrow_val_tuple.0.v == vs[0] == bound_val_tuple.0.v;
-
-            var new_index := index + SizeOfV(narrow_val_tuple.0.v);
-            calc {
-                SizeOfV(narrow_val_tuple.0.v) + SeqSum(vs[1..]);
-                    { reveal_SeqSum(); }
-                SeqSum(vs);
-            }
-            assert new_index+SeqSum(vs[1..]) <= bound;
-
-            lemma_parse_Val_view_Array_contents(data, vs[1..], grammar, new_index, bound, len - 1);
-
-            assert (parse_Array_contents(data[new_index..bound], grammar, len - 1).0 == Some(vs[1..])) <==> (parse_Array_contents(data[new_index..new_index+SeqSum(vs[1..])], grammar, len - 1).0 == Some(vs[1..]));
-            assert data[new_index..new_index+SeqSum(vs[1..])] == narrow_val_tuple.1;
-            assert data[new_index..bound] == bound_val_tuple.1;
-
-            assert narrow_tuple.0 == Some([vs[0]] + vs[1..]) == Some(vs);
-        } else {
-            // Doesn't matter for our ensures clause
-        }
+      // Doesn't matter for our ensures clause
     }
+  }
 }
 
 lemma lemma_parse_Val_view_Array(data:seq<byte>, v:V, grammar:G, index:int, bound:int)
-    requires |data| < 0x1_0000_0000_0000_0000;
-    requires ValInGrammar(v, grammar);
-    requires ValidGrammar(grammar);
-    requires grammar.GArray?;
-    requires 0 <= index <= |data|;
-    requires 0 <= index + SizeOfV(v) <= |data|;
-    requires index+SizeOfV(v) <= bound <= |data|;
-    decreases grammar, -1;
-    ensures  (parse_Array(data[index..bound], grammar.elt).0 == Some(v)) <==> (parse_Array(data[index..index+SizeOfV(v)], grammar.elt).0 == Some(v));
-    ensures  parse_Array(data[index..bound], grammar.elt).0 == Some(v) ==> parse_Array(data[index..bound], grammar.elt).1 == data[index+SizeOfV(v)..bound];
+  requires |data| < 0x1_0000_0000_0000_0000
+  requires ValInGrammar(v, grammar)
+  requires ValidGrammar(grammar)
+  requires grammar.GArray?
+  requires 0 <= index <= |data|
+  requires 0 <= index + SizeOfV(v) <= |data|
+  requires index+SizeOfV(v) <= bound <= |data|
+  decreases grammar, -1
+  ensures  (parse_Array(data[index..bound], grammar.elt).0 == Some(v)) <==> (parse_Array(data[index..index+SizeOfV(v)], grammar.elt).0 == Some(v))
+  ensures  parse_Array(data[index..bound], grammar.elt).0 == Some(v) ==> parse_Array(data[index..bound], grammar.elt).1 == data[index+SizeOfV(v)..bound]
 {
-    var narrow_tuple := parse_Array(data[index..index+SizeOfV(v)], grammar.elt);
-    var bound_tuple := parse_Array(data[index..bound], grammar.elt);
-    var narrow_len_tuple := parse_Uint64(data[index..index+SizeOfV(v)]);
-    var bound_len_tuple := parse_Uint64(data[index..bound]);
-    var narrow_contents_tuple := parse_Array_contents(narrow_len_tuple.1, grammar.elt, narrow_len_tuple.0.v.u);
-    var bound_contents_tuple := parse_Array_contents(bound_len_tuple.1, grammar.elt, bound_len_tuple.0.v.u);
+  var narrow_tuple := parse_Array(data[index..index+SizeOfV(v)], grammar.elt);
+  var bound_tuple := parse_Array(data[index..bound], grammar.elt);
+  var narrow_len_tuple := parse_Uint64(data[index..index+SizeOfV(v)]);
+  var bound_len_tuple := parse_Uint64(data[index..bound]);
+  var narrow_contents_tuple := parse_Array_contents(narrow_len_tuple.1, grammar.elt, narrow_len_tuple.0.v.u);
+  var bound_contents_tuple := parse_Array_contents(bound_len_tuple.1, grammar.elt, bound_len_tuple.0.v.u);
 
-    assert narrow_len_tuple.0 == bound_len_tuple.0;
+  assert narrow_len_tuple.0 == bound_len_tuple.0;
 
-    if bound_tuple.0 == Some(v) {
-        assert parse_Array_contents(bound_len_tuple.1, grammar.elt, bound_len_tuple.0.v.u).0 == Some(v.a);   // OBSERVE
-        lemma_parse_Array_contents_len(bound_len_tuple.1, grammar.elt, narrow_len_tuple.0.v.u);
-        lemma_parse_Val_view_Array_contents(data, v.a, grammar.elt, index+8, bound, narrow_len_tuple.0.v.u);
-    }
+  if bound_tuple.0 == Some(v) {
+    assert parse_Array_contents(bound_len_tuple.1, grammar.elt, bound_len_tuple.0.v.u).0 == Some(v.a);   // OBSERVE
+    lemma_parse_Array_contents_len(bound_len_tuple.1, grammar.elt, narrow_len_tuple.0.v.u);
+    lemma_parse_Val_view_Array_contents(data, v.a, grammar.elt, index+8, bound, narrow_len_tuple.0.v.u);
+  }
 
-    if narrow_tuple.0 == Some(v) {
-        assert parse_Array_contents(narrow_len_tuple.1, grammar.elt, narrow_len_tuple.0.v.u).0 == Some(v.a);   // OBSERVE
-        lemma_parse_Array_contents_len(narrow_len_tuple.1, grammar.elt, narrow_len_tuple.0.v.u);
-        lemma_parse_Val_view_Array_contents(data, v.a, grammar.elt, index+8, bound, narrow_len_tuple.0.v.u);
-    }
+  if narrow_tuple.0 == Some(v) {
+    assert parse_Array_contents(narrow_len_tuple.1, grammar.elt, narrow_len_tuple.0.v.u).0 == Some(v.a);   // OBSERVE
+    lemma_parse_Array_contents_len(narrow_len_tuple.1, grammar.elt, narrow_len_tuple.0.v.u);
+    lemma_parse_Val_view_Array_contents(data, v.a, grammar.elt, index+8, bound, narrow_len_tuple.0.v.u);
+  }
 }
 
 lemma lemma_parse_Val_view_Tuple_contents(data:seq<byte>, vs:seq<V>, grammar:seq<G>, index:int, bound:int)
-    requires |data| < 0x1_0000_0000_0000_0000;
-    requires |vs| == |grammar|;
-    requires forall i :: 0 <= i < |vs| ==> ValInGrammar(vs[i], grammar[i]);
-    requires |grammar| < 0x1_0000_0000_0000_0000;
-    requires forall g :: g in grammar ==> ValidGrammar(g);
-    requires 0 <= index <= |data|;
-    requires 0 <= index + SeqSum(vs) <= |data|;
-    requires index+SeqSum(vs) <= bound <= |data|;
-    decreases grammar, -1, vs;
-    ensures  (parse_Tuple_contents(data[index..bound], grammar).0 == Some(vs)) <==> (parse_Tuple_contents(data[index..index+SeqSum(vs)], grammar).0 == Some(vs));
-    ensures  parse_Tuple_contents(data[index..bound], grammar).0 == Some(vs) ==> parse_Tuple_contents(data[index..bound], grammar).1 == data[index+SeqSum(vs)..bound];
+  requires |data| < 0x1_0000_0000_0000_0000
+  requires |vs| == |grammar|
+  requires forall i :: 0 <= i < |vs| ==> ValInGrammar(vs[i], grammar[i])
+  requires |grammar| < 0x1_0000_0000_0000_0000
+  requires forall g :: g in grammar ==> ValidGrammar(g)
+  requires 0 <= index <= |data|
+  requires 0 <= index + SeqSum(vs) <= |data|
+  requires index+SeqSum(vs) <= bound <= |data|
+  decreases grammar, -1, vs
+  ensures  (parse_Tuple_contents(data[index..bound], grammar).0 == Some(vs)) <==> (parse_Tuple_contents(data[index..index+SeqSum(vs)], grammar).0 == Some(vs))
+  ensures  parse_Tuple_contents(data[index..bound], grammar).0 == Some(vs) ==> parse_Tuple_contents(data[index..bound], grammar).1 == data[index+SeqSum(vs)..bound]
 {
-    reveal_parse_Tuple_contents();
-    if grammar == [] {
-        reveal_SeqSum();
-    } else {
-        var narrow_tuple := parse_Tuple_contents(data[index..index+SeqSum(vs)], grammar);
-        var bound_tuple := parse_Tuple_contents(data[index..bound], grammar);
-        var narrow_val_tuple := parse_Val(data[index..index+SeqSum(vs)], grammar[0]);
-        var bound_val_tuple := parse_Val(data[index..bound], grammar[0]);
-        var narrow_contents_tuple := parse_Tuple_contents(narrow_val_tuple.1, grammar[1..]);
-        var bound_contents_tuple := parse_Tuple_contents(bound_val_tuple.1, grammar[1..]);
+  reveal parse_Tuple_contents();
+  if grammar == [] {
+    reveal SeqSum();
+  } else {
+    var narrow_tuple := parse_Tuple_contents(data[index..index+SeqSum(vs)], grammar);
+    var bound_tuple := parse_Tuple_contents(data[index..bound], grammar);
+    var narrow_val_tuple := parse_Val(data[index..index+SeqSum(vs)], grammar[0]);
+    var bound_val_tuple := parse_Val(data[index..bound], grammar[0]);
+    var narrow_contents_tuple := parse_Tuple_contents(narrow_val_tuple.1, grammar[1..]);
+    var bound_contents_tuple := parse_Tuple_contents(bound_val_tuple.1, grammar[1..]);
 
 
-        if narrow_tuple.0 == Some(vs) {
-            assert !narrow_val_tuple.0.None? && !narrow_contents_tuple.0.None?;
-            calc {
-                index + SeqSum(vs) <= |data|;
-                SeqSum(vs) <= |data| - index;
-                SeqSum(vs) < |data| - index + 1;
-            }
-            lemma_SeqSum_bound(vs, |data| - index + 1);
-            lemma_parse_Val_view(data, vs[0], grammar[0], index);
-            lemma_SeqSum_bound(vs, SeqSum(vs) + 1);
-            assert index+SizeOfV(vs[0]) <= bound <= |data|;
-            assert (parse_Val(data[index..index+SeqSum(vs)], grammar[0]).0 == Some(vs[0])) <==> (parse_Val(data[index..index+SizeOfV(vs[0])], grammar[0]).0 == Some(vs[0]));
-            lemma_SeqSum_bound(vs, bound - index + 1);
-            assert index+SizeOfV(vs[0]) <= bound <= |data|;     // OBSERVE (trigger on forall?)
-            assert (parse_Val(data[index..bound], grammar[0]).0 == Some(vs[0])) <==> (parse_Val(data[index..index+SizeOfV(vs[0])], grammar[0]).0 == Some(vs[0]));
-            assert narrow_val_tuple.0.v == vs[0] == bound_val_tuple.0.v;
+    if narrow_tuple.0 == Some(vs) {
+      assert !narrow_val_tuple.0.None? && !narrow_contents_tuple.0.None?;
+      calc {
+        index + SeqSum(vs) <= |data|;
+        SeqSum(vs) <= |data| - index;
+        SeqSum(vs) < |data| - index + 1;
+      }
+      lemma_SeqSum_bound(vs, |data| - index + 1);
+      lemma_parse_Val_view(data, vs[0], grammar[0], index);
+      lemma_SeqSum_bound(vs, SeqSum(vs) + 1);
+      assert index+SizeOfV(vs[0]) <= bound <= |data|;
+      assert (parse_Val(data[index..index+SeqSum(vs)], grammar[0]).0 == Some(vs[0])) <==> (parse_Val(data[index..index+SizeOfV(vs[0])], grammar[0]).0 == Some(vs[0]));
+      lemma_SeqSum_bound(vs, bound - index + 1);
+      assert index+SizeOfV(vs[0]) <= bound <= |data|;     // OBSERVE (trigger on forall?)
+      assert (parse_Val(data[index..bound], grammar[0]).0 == Some(vs[0])) <==> (parse_Val(data[index..index+SizeOfV(vs[0])], grammar[0]).0 == Some(vs[0]));
+      assert narrow_val_tuple.0.v == vs[0] == bound_val_tuple.0.v;
 
-            var new_index := index + SizeOfV(narrow_val_tuple.0.v);
-            calc {
-                SizeOfV(narrow_val_tuple.0.v) + SeqSum(vs[1..]);
-                    { reveal_SeqSum(); }
-                SeqSum(vs);
-            }
-            assert new_index+SeqSum(vs[1..]) <= bound;
+      var new_index := index + SizeOfV(narrow_val_tuple.0.v);
+      calc {
+        SizeOfV(narrow_val_tuple.0.v) + SeqSum(vs[1..]);
+          { reveal SeqSum(); }
+        SeqSum(vs);
+      }
+      assert new_index+SeqSum(vs[1..]) <= bound;
 
-            lemma_parse_Val_view_Tuple_contents(data, vs[1..], grammar[1..], new_index, bound);
+      lemma_parse_Val_view_Tuple_contents(data, vs[1..], grammar[1..], new_index, bound);
 
-            assert (parse_Tuple_contents(data[new_index..bound], grammar[1..]).0 == Some(vs[1..])) <==> (parse_Tuple_contents(data[new_index..new_index+SeqSum(vs[1..])], grammar[1..]).0 == Some(vs[1..]));
-            assert data[new_index..new_index+SeqSum(vs[1..])] == narrow_val_tuple.1;
-            assert data[new_index..bound] == bound_val_tuple.1;
+      assert (parse_Tuple_contents(data[new_index..bound], grammar[1..]).0 == Some(vs[1..])) <==> (parse_Tuple_contents(data[new_index..new_index+SeqSum(vs[1..])], grammar[1..]).0 == Some(vs[1..]));
+      assert data[new_index..new_index+SeqSum(vs[1..])] == narrow_val_tuple.1;
+      assert data[new_index..bound] == bound_val_tuple.1;
 
-            assert bound_tuple.0 == Some([vs[0]] + vs[1..]) == Some(vs);
-        } else if bound_tuple.0 == Some(vs) {
-            assert !bound_val_tuple.0.None? && !bound_contents_tuple.0.None?;
+      assert bound_tuple.0 == Some([vs[0]] + vs[1..]) == Some(vs);
+    } else if bound_tuple.0 == Some(vs) {
+      assert !bound_val_tuple.0.None? && !bound_contents_tuple.0.None?;
 
-            lemma_SeqSum_bound(vs, |data| - index + 1);
-            lemma_parse_Val_view(data, vs[0], grammar[0], index);
-            // This is exactly the ensures of the lemma above
-            assert forall bound' :: index+SizeOfV(vs[0]) <= bound' <= |data| ==>
+      lemma_SeqSum_bound(vs, |data| - index + 1);
+      lemma_parse_Val_view(data, vs[0], grammar[0], index);
+      // This is exactly the ensures of the lemma above
+      assert forall bound' :: index+SizeOfV(vs[0]) <= bound' <= |data| ==>
                    ((parse_Val(data[index..bound'], grammar[0]).0 == Some(vs[0])) <==> (parse_Val(data[index..index+SizeOfV(vs[0])], grammar[0]).0 == Some(vs[0])));
 
-            lemma_SeqSum_bound(vs, bound - index + 1);
-            lemma_SeqSum_bound(vs, SeqSum(vs) + 1);
-            assert index+SizeOfV(vs[0]) <= index+SeqSum(vs) <= |data|;
-            assert (parse_Val(data[index..index+SeqSum(vs)], grammar[0]).0 == Some(vs[0])) <==> (parse_Val(data[index..index+SizeOfV(vs[0])], grammar[0]).0 == Some(vs[0]));
-            assert (parse_Val(data[index..bound], grammar[0]).0 == Some(vs[0])) <==> (parse_Val(data[index..index+SizeOfV(vs[0])], grammar[0]).0 == Some(vs[0]));
-            assert narrow_val_tuple.0.v == vs[0] == bound_val_tuple.0.v;
+      lemma_SeqSum_bound(vs, bound - index + 1);
+      lemma_SeqSum_bound(vs, SeqSum(vs) + 1);
+      assert index+SizeOfV(vs[0]) <= index+SeqSum(vs) <= |data|;
+      assert (parse_Val(data[index..index+SeqSum(vs)], grammar[0]).0 == Some(vs[0])) <==> (parse_Val(data[index..index+SizeOfV(vs[0])], grammar[0]).0 == Some(vs[0]));
+      assert (parse_Val(data[index..bound], grammar[0]).0 == Some(vs[0])) <==> (parse_Val(data[index..index+SizeOfV(vs[0])], grammar[0]).0 == Some(vs[0]));
+      assert narrow_val_tuple.0.v == vs[0] == bound_val_tuple.0.v;
 
-            var new_index := index + SizeOfV(narrow_val_tuple.0.v);
-            calc {
-                SizeOfV(narrow_val_tuple.0.v) + SeqSum(vs[1..]);
-                    { reveal_SeqSum(); }
-                SeqSum(vs);
-            }
-            assert new_index+SeqSum(vs[1..]) <= bound;
+      var new_index := index + SizeOfV(narrow_val_tuple.0.v);
+      calc {
+        SizeOfV(narrow_val_tuple.0.v) + SeqSum(vs[1..]);
+          { reveal SeqSum(); }
+        SeqSum(vs);
+      }
+      assert new_index+SeqSum(vs[1..]) <= bound;
 
-            lemma_parse_Val_view_Tuple_contents(data, vs[1..], grammar[1..], new_index, bound);
+      lemma_parse_Val_view_Tuple_contents(data, vs[1..], grammar[1..], new_index, bound);
 
-            assert (parse_Tuple_contents(data[new_index..bound], grammar[1..]).0 == Some(vs[1..])) <==> (parse_Tuple_contents(data[new_index..new_index+SeqSum(vs[1..])], grammar[1..]).0 == Some(vs[1..]));
-            assert data[new_index..new_index+SeqSum(vs[1..])] == narrow_val_tuple.1;
-            assert data[new_index..bound] == bound_val_tuple.1;
+      assert (parse_Tuple_contents(data[new_index..bound], grammar[1..]).0 == Some(vs[1..])) <==> (parse_Tuple_contents(data[new_index..new_index+SeqSum(vs[1..])], grammar[1..]).0 == Some(vs[1..]));
+      assert data[new_index..new_index+SeqSum(vs[1..])] == narrow_val_tuple.1;
+      assert data[new_index..bound] == bound_val_tuple.1;
 
-            assert narrow_tuple.0 == Some([vs[0]] + vs[1..]) == Some(vs);
-        } else {
-            // Doesn't matter for our ensures clause
-        }
+      assert narrow_tuple.0 == Some([vs[0]] + vs[1..]) == Some(vs);
+    } else {
+      // Doesn't matter for our ensures clause
     }
-
+  }
 }
 
 lemma lemma_parse_Val_view_Tuple(data:seq<byte>, v:V, grammar:seq<G>, index:int, bound:int)
-    requires |data| < 0x1_0000_0000_0000_0000;
-    requires v.VTuple?;
-    requires |v.t| == |grammar|
-    requires forall i :: 0 <= i < |v.t| ==> ValInGrammar(v.t[i], grammar[i]);
-    requires |grammar| < 0x1_0000_0000_0000_0000;
-    requires forall g :: g in grammar ==> ValidGrammar(g);
-    requires 0 <= index <= |data|;
-    requires 0 <= index + SizeOfV(v) <= |data|;
-    requires index+SizeOfV(v) <= bound <= |data|;
-    decreases grammar, -1, v;
-    ensures  (parse_Tuple(data[index..bound], grammar).0 == Some(v)) <==> (parse_Tuple(data[index..index+SizeOfV(v)], grammar).0 == Some(v));
-    ensures  parse_Tuple(data[index..bound], grammar).0 == Some(v) ==> parse_Tuple(data[index..bound], grammar).1 == data[index+SizeOfV(v)..bound];
+  requires |data| < 0x1_0000_0000_0000_0000
+  requires v.VTuple?
+  requires |v.t| == |grammar|
+  requires forall i :: 0 <= i < |v.t| ==> ValInGrammar(v.t[i], grammar[i])
+  requires |grammar| < 0x1_0000_0000_0000_0000
+  requires forall g :: g in grammar ==> ValidGrammar(g)
+  requires 0 <= index <= |data|
+  requires 0 <= index + SizeOfV(v) <= |data|
+  requires index+SizeOfV(v) <= bound <= |data|
+  decreases grammar, -1, v
+  ensures  (parse_Tuple(data[index..bound], grammar).0 == Some(v)) <==> (parse_Tuple(data[index..index+SizeOfV(v)], grammar).0 == Some(v))
+  ensures  parse_Tuple(data[index..bound], grammar).0 == Some(v) ==> parse_Tuple(data[index..bound], grammar).1 == data[index+SizeOfV(v)..bound]
 {
-    var bound_tuple := parse_Tuple(data[index..bound], grammar);
-    var bound_contents := bound_tuple.0;
-    var bound_rest := bound_tuple.1;
-    var narrow_tuple := parse_Tuple(data[index..index+SizeOfV(v)], grammar);
-    var narrow_contents := narrow_tuple.0;
-    var narrow_rest := narrow_tuple.1;
+  var bound_tuple := parse_Tuple(data[index..bound], grammar);
+  var bound_contents := bound_tuple.0;
+  var bound_rest := bound_tuple.1;
+  var narrow_tuple := parse_Tuple(data[index..index+SizeOfV(v)], grammar);
+  var narrow_contents := narrow_tuple.0;
+  var narrow_rest := narrow_tuple.1;
 
-    if parse_Tuple(data[index..bound], grammar).0 == Some(v) {
-        assert !bound_contents.None?;
-        lemma_parse_Val_view_Tuple_contents(data, v.t, grammar, index, bound);
-        assert (parse_Tuple_contents(data[index..bound], grammar).0 == Some(v.t)) <==> (parse_Tuple_contents(data[index..index+SeqSum(v.t)], grammar).0 == Some(v.t)); // OBSERVE
-    } else if parse_Tuple(data[index..index+SizeOfV(v)], grammar).0 == Some(v) {
-        assert !narrow_contents.None?;
-        lemma_parse_Val_view_Tuple_contents(data, v.t, grammar, index, bound);
-        assert (parse_Tuple_contents(data[index..bound], grammar).0 == Some(v.t)) <==> (parse_Tuple_contents(data[index..index+SeqSum(v.t)], grammar).0 == Some(v.t)); // OBSERVE
-    } else {
-        // Don't care
-    }
+  if parse_Tuple(data[index..bound], grammar).0 == Some(v) {
+    assert !bound_contents.None?;
+    lemma_parse_Val_view_Tuple_contents(data, v.t, grammar, index, bound);
+    assert (parse_Tuple_contents(data[index..bound], grammar).0 == Some(v.t)) <==> (parse_Tuple_contents(data[index..index+SeqSum(v.t)], grammar).0 == Some(v.t)); // OBSERVE
+  } else if parse_Tuple(data[index..index+SizeOfV(v)], grammar).0 == Some(v) {
+    assert !narrow_contents.None?;
+    lemma_parse_Val_view_Tuple_contents(data, v.t, grammar, index, bound);
+    assert (parse_Tuple_contents(data[index..bound], grammar).0 == Some(v.t)) <==> (parse_Tuple_contents(data[index..index+SeqSum(v.t)], grammar).0 == Some(v.t)); // OBSERVE
+  } else {
+    // Don't care
+  }
 }
 
 lemma lemma_parse_Val_view_Union(data:seq<byte>, v:V, grammar:G, index:int, bound:int)
-    requires |data| < 0x1_0000_0000_0000_0000;
-    requires ValInGrammar(v, grammar);
-    requires ValidGrammar(grammar);
-    requires grammar.GTaggedUnion?;
-    requires 0 <= index <= |data|;
-    requires 0 <= index + SizeOfV(v) <= |data|;
-    requires index+SizeOfV(v) <= bound <= |data|;
-    decreases grammar, -1;
-    ensures  (parse_Case(data[index..bound], grammar.cases).0 == Some(v)) <==> (parse_Case(data[index..index+SizeOfV(v)], grammar.cases).0 == Some(v));
-    ensures  parse_Case(data[index..bound], grammar.cases).0 == Some(v) ==> parse_Case(data[index..bound], grammar.cases).1 == data[index+SizeOfV(v)..bound];
+  requires |data| < 0x1_0000_0000_0000_0000
+  requires ValInGrammar(v, grammar)
+  requires ValidGrammar(grammar)
+  requires grammar.GTaggedUnion?
+  requires 0 <= index <= |data|
+  requires 0 <= index + SizeOfV(v) <= |data|
+  requires index+SizeOfV(v) <= bound <= |data|
+  decreases grammar, -1
+  ensures  (parse_Case(data[index..bound], grammar.cases).0 == Some(v)) <==> (parse_Case(data[index..index+SizeOfV(v)], grammar.cases).0 == Some(v))
+  ensures  parse_Case(data[index..bound], grammar.cases).0 == Some(v) ==> parse_Case(data[index..bound], grammar.cases).1 == data[index+SizeOfV(v)..bound]
 {
-    var narrow_tuple := parse_Case(data[index..index+SizeOfV(v)], grammar.cases);
-    var bound_tuple := parse_Case(data[index..bound], grammar.cases);
-    var narrow_caseID_tuple := parse_Uint64(data[index..index+SizeOfV(v)]);
-    var bound_caseID_tuple := parse_Uint64(data[index..bound]);
-    // assert narrow_caseID_tuple.0.v == bound_caseID_tuple.0.v;
+  var narrow_tuple := parse_Case(data[index..index+SizeOfV(v)], grammar.cases);
+  var bound_tuple := parse_Case(data[index..bound], grammar.cases);
+  var narrow_caseID_tuple := parse_Uint64(data[index..index+SizeOfV(v)]);
+  var bound_caseID_tuple := parse_Uint64(data[index..bound]);
+  // assert narrow_caseID_tuple.0.v == bound_caseID_tuple.0.v;
 
-    if parse_Case(data[index..bound], grammar.cases).0 == Some(v) {
-        var narrow_val_tuple := parse_Val(narrow_caseID_tuple.1, grammar.cases[narrow_caseID_tuple.0.v.u]);
-        var bound_val_tuple := parse_Val(bound_caseID_tuple.1, grammar.cases[bound_caseID_tuple.0.v.u]);
+  if parse_Case(data[index..bound], grammar.cases).0 == Some(v) {
+    var narrow_val_tuple := parse_Val(narrow_caseID_tuple.1, grammar.cases[narrow_caseID_tuple.0.v.u]);
+    var bound_val_tuple := parse_Val(bound_caseID_tuple.1, grammar.cases[bound_caseID_tuple.0.v.u]);
 
-        // assert ValInGrammar(v.val, grammar.cases[narrow_caseID_tuple.0.v.u]);
-        if (ValInGrammar(v.val, grammar.cases[narrow_caseID_tuple.0.v.u])){
-        lemma_parse_Val_view(data, v.val, grammar.cases[narrow_caseID_tuple.0.v.u], index + 8);
-        assert index+SizeOfV(v.val) <= bound <= |data|;
-        assert (parse_Val(data[index+8..bound], grammar.cases[narrow_caseID_tuple.0.v.u]).0 == Some(v.val)) <==> (parse_Val(data[index+8..index+8+SizeOfV(v.val)], grammar.cases[narrow_caseID_tuple.0.v.u]).0 == Some(v.val));
-        }
-    } else if parse_Case(data[index..index+SizeOfV(v)], grammar.cases).0 == Some(v) {
-        var narrow_val_tuple := parse_Val(narrow_caseID_tuple.1, grammar.cases[narrow_caseID_tuple.0.v.u]);
-        // var bound_val_tuple := parse_Val(bound_caseID_tuple.1, grammar.cases[bound_caseID_tuple.0.v.u]);
-
-        lemma_parse_Val_view(data, v.val, grammar.cases[narrow_caseID_tuple.0.v.u], index + 8);
-        assert (parse_Val(data[index+8..bound], grammar.cases[narrow_caseID_tuple.0.v.u]).0 == Some(v.val)) <==> (parse_Val(data[index+8..index+8+SizeOfV(v.val)], grammar.cases[narrow_caseID_tuple.0.v.u]).0 == Some(v.val));
-    } else {
-        // Doesn't matter
+    // assert ValInGrammar(v.val, grammar.cases[narrow_caseID_tuple.0.v.u]);
+    if (ValInGrammar(v.val, grammar.cases[narrow_caseID_tuple.0.v.u])){
+      lemma_parse_Val_view(data, v.val, grammar.cases[narrow_caseID_tuple.0.v.u], index + 8);
+      assert index+SizeOfV(v.val) <= bound <= |data|;
+      assert (parse_Val(data[index+8..bound], grammar.cases[narrow_caseID_tuple.0.v.u]).0 == Some(v.val)) <==> (parse_Val(data[index+8..index+8+SizeOfV(v.val)], grammar.cases[narrow_caseID_tuple.0.v.u]).0 == Some(v.val));
     }
+  } else if parse_Case(data[index..index+SizeOfV(v)], grammar.cases).0 == Some(v) {
+    var narrow_val_tuple := parse_Val(narrow_caseID_tuple.1, grammar.cases[narrow_caseID_tuple.0.v.u]);
+    // var bound_val_tuple := parse_Val(bound_caseID_tuple.1, grammar.cases[bound_caseID_tuple.0.v.u]);
+
+    lemma_parse_Val_view(data, v.val, grammar.cases[narrow_caseID_tuple.0.v.u], index + 8);
+    assert (parse_Val(data[index+8..bound], grammar.cases[narrow_caseID_tuple.0.v.u]).0 == Some(v.val)) <==> (parse_Val(data[index+8..index+8+SizeOfV(v.val)], grammar.cases[narrow_caseID_tuple.0.v.u]).0 == Some(v.val));
+  } else {
+    // Doesn't matter
+  }
 }
 
 lemma lemma_parse_Val_view(data:seq<byte>, v:V, grammar:G, index:int)
-    requires |data| < 0x1_0000_0000_0000_0000;
-    requires ValInGrammar(v, grammar);
-    requires ValidGrammar(grammar);
-    requires 0 <= index <= |data|;
-    requires 0 <= index + SizeOfV(v) <= |data|;
-    decreases grammar, 0;
-    ensures  forall bound :: index+SizeOfV(v) <= bound <= |data| ==>
-             ((parse_Val(data[index..bound], grammar).0 == Some(v)) <==> (parse_Val(data[index..index+SizeOfV(v)], grammar).0 == Some(v)));
-    ensures  forall bound :: index+SizeOfV(v) <= bound <= |data| ==>
-             (parse_Val(data[index..bound], grammar).0 == Some(v)) ==> parse_Val(data[index..bound], grammar).1 == data[index+SizeOfV(v)..bound];
+  requires |data| < 0x1_0000_0000_0000_0000
+  requires ValInGrammar(v, grammar)
+  requires ValidGrammar(grammar)
+  requires 0 <= index <= |data|
+  requires 0 <= index + SizeOfV(v) <= |data|
+  decreases grammar, 0
+  ensures  forall bound :: index+SizeOfV(v) <= bound <= |data| ==>
+             ((parse_Val(data[index..bound], grammar).0 == Some(v)) <==> (parse_Val(data[index..index+SizeOfV(v)], grammar).0 == Some(v)))
+  ensures  forall bound :: index+SizeOfV(v) <= bound <= |data| ==>
+             (parse_Val(data[index..bound], grammar).0 == Some(v)) ==> parse_Val(data[index..bound], grammar).1 == data[index+SizeOfV(v)..bound]
 {
-    forall bound | index+SizeOfV(v) <= bound <= |data|
-         ensures (parse_Val(data[index..bound], grammar).0 == Some(v)) <==> (parse_Val(data[index..index+SizeOfV(v)], grammar).0 == Some(v));
-         ensures (parse_Val(data[index..bound], grammar).0 == Some(v)) ==> parse_Val(data[index..bound], grammar).1 == data[index+SizeOfV(v)..bound];
-    {
-        reveal_parse_Val();
-        match grammar
-            case GUint64             => assert (parse_Val(data[index..bound], grammar).0 == Some(v)) <==> (parse_Val(data[index..index+SizeOfV(v)], grammar).0 == Some(v));
-            case GArray(elt)         => lemma_parse_Val_view_Array(data, v, grammar, index, bound);
-                                        assert (parse_Val(data[index..bound], grammar).0 == Some(v)) <==> (parse_Val(data[index..index+SizeOfV(v)], grammar).0 == Some(v));
-            case GTuple(t)           => lemma_parse_Val_view_Tuple(data, v, t, index, bound); assert (parse_Val(data[index..bound], grammar).0 == Some(v)) <==> (parse_Val(data[index..index+SizeOfV(v)], grammar).0 == Some(v));
-            case GByteArray          => lemma_parse_Val_view_ByteArray(data, v, grammar, index); assert (parse_Val(data[index..bound], grammar).0 == Some(v)) <==> (parse_Val(data[index..index+SizeOfV(v)], grammar).0 == Some(v));
-            case GTaggedUnion(cases) => lemma_parse_Val_view_Union(data, v, grammar, index, bound); assert (parse_Val(data[index..bound], grammar).0 == Some(v)) <==> (parse_Val(data[index..index+SizeOfV(v)], grammar).0 == Some(v));
-
-    }
+  forall bound | index+SizeOfV(v) <= bound <= |data|
+    ensures (parse_Val(data[index..bound], grammar).0 == Some(v)) <==> (parse_Val(data[index..index+SizeOfV(v)], grammar).0 == Some(v))
+    ensures (parse_Val(data[index..bound], grammar).0 == Some(v)) ==> parse_Val(data[index..bound], grammar).1 == data[index+SizeOfV(v)..bound]
+  {
+    reveal parse_Val();
+    match grammar
+      case GUint64             => assert (parse_Val(data[index..bound], grammar).0 == Some(v)) <==> (parse_Val(data[index..index+SizeOfV(v)], grammar).0 == Some(v));
+      case GArray(elt)         => lemma_parse_Val_view_Array(data, v, grammar, index, bound);
+                                  assert (parse_Val(data[index..bound], grammar).0 == Some(v)) <==> (parse_Val(data[index..index+SizeOfV(v)], grammar).0 == Some(v));
+      case GTuple(t)           => lemma_parse_Val_view_Tuple(data, v, t, index, bound); assert (parse_Val(data[index..bound], grammar).0 == Some(v)) <==> (parse_Val(data[index..index+SizeOfV(v)], grammar).0 == Some(v));
+      case GByteArray          => lemma_parse_Val_view_ByteArray(data, v, grammar, index); assert (parse_Val(data[index..bound], grammar).0 == Some(v)) <==> (parse_Val(data[index..index+SizeOfV(v)], grammar).0 == Some(v));
+      case GTaggedUnion(cases) => lemma_parse_Val_view_Union(data, v, grammar, index, bound); assert (parse_Val(data[index..bound], grammar).0 == Some(v)) <==> (parse_Val(data[index..index+SizeOfV(v)], grammar).0 == Some(v));
+  }
 }
 
 
 lemma lemma_parse_Val_view_specific(data:seq<byte>, v:V, grammar:G, index:int, bound:int)
-    requires |data| < 0x1_0000_0000_0000_0000;
-    requires ValInGrammar(v, grammar);
-    requires ValidGrammar(grammar);
-    requires 0 <= index <= |data|;
-    requires 0 <= index + SizeOfV(v) <= |data|;
-    requires index+SizeOfV(v) <= bound <= |data|; 
-    requires parse_Val(data[index..index+SizeOfV(v)], grammar).0 == Some(v)
-    decreases grammar, 0;
-    ensures  parse_Val(data[index..bound], grammar).0 == Some(v);
-    ensures  parse_Val(data[index..bound], grammar).1 == data[index+SizeOfV(v)..bound];
+  requires |data| < 0x1_0000_0000_0000_0000
+  requires ValInGrammar(v, grammar)
+  requires ValidGrammar(grammar)
+  requires 0 <= index <= |data|
+  requires 0 <= index + SizeOfV(v) <= |data|
+  requires index+SizeOfV(v) <= bound <= |data|;
+  requires parse_Val(data[index..index+SizeOfV(v)], grammar).0 == Some(v)
+  decreases grammar, 0
+  ensures  parse_Val(data[index..bound], grammar).0 == Some(v)
+  ensures  parse_Val(data[index..bound], grammar).1 == data[index+SizeOfV(v)..bound]
 {
-    lemma_parse_Val_view(data, v, grammar, index);
+  lemma_parse_Val_view(data, v, grammar, index);
 }
 
 lemma lemma_parse_Val_view_specific_size(data:seq<byte>, v:V, grammar:G, index:int, bound:int)
-    requires |data| < 0x1_0000_0000_0000_0000;
-    requires ValInGrammar(v, grammar);
-    requires ValidGrammar(grammar);
-    requires 0 <= index <= |data|;
-    requires 0 <= index + SizeOfV(v) <= |data|;
-    requires index+SizeOfV(v) <= bound <= |data|; 
-    requires parse_Val(data[index..bound], grammar).0 == Some(v)
-    decreases grammar, 0;
-    ensures  parse_Val(data[index..index+SizeOfV(v)], grammar).0 == Some(v);
-    ensures  parse_Val(data[index..bound], grammar).1 == data[index+SizeOfV(v)..bound];
+  requires |data| < 0x1_0000_0000_0000_0000
+  requires ValInGrammar(v, grammar)
+  requires ValidGrammar(grammar)
+  requires 0 <= index <= |data|
+  requires 0 <= index + SizeOfV(v) <= |data|
+  requires index+SizeOfV(v) <= bound <= |data|;
+  requires parse_Val(data[index..bound], grammar).0 == Some(v)
+  decreases grammar, 0
+  ensures  parse_Val(data[index..index+SizeOfV(v)], grammar).0 == Some(v)
+  ensures  parse_Val(data[index..bound], grammar).1 == data[index+SizeOfV(v)..bound]
 {
-    lemma_parse_Val_view(data, v, grammar, index);
+  lemma_parse_Val_view(data, v, grammar, index);
 }
 
 method ComputeSeqSum(s:seq<V>) returns (size:uint64)
-    requires |s| < 0x1_0000_0000_0000_0000;
-    requires 0 <= SeqSum(s) < 0x1_0000_0000_0000_0000;
-    requires forall v :: v in s ==> ValidVal(v);
-    ensures int(size) == SeqSum(s);
+  requires |s| < 0x1_0000_0000_0000_0000
+  requires 0 <= SeqSum(s) < 0x1_0000_0000_0000_0000
+  requires forall v :: v in s ==> ValidVal(v)
+  ensures size as int == SeqSum(s)
 {
-    reveal_SeqSum();
-    if uint64(|s|) == 0 {
-        size := 0;
-    } else {
-        var v_size := ComputeSizeOf(s[uint64(0)]);
-        var rest_size := ComputeSeqSum(s[uint64(1)..]);
-        size := v_size + rest_size;
-    }
+  reveal SeqSum();
+  if |s| as uint64 == 0 {
+    size := 0;
+  } else {
+    var v_size := ComputeSizeOf(s[0]);
+    var rest_size := ComputeSeqSum(s[1..]);
+    size := v_size + rest_size;
+  }
 }
 
 method ComputeSizeOf(val:V) returns (size:uint64)
-    requires 0 <= SizeOfV(val) < 0x1_0000_0000_0000_0000;
-    requires ValidVal(val);
-    ensures int(size) == SizeOfV(val);
+  requires 0 <= SizeOfV(val) < 0x1_0000_0000_0000_0000
+  requires ValidVal(val)
+  ensures size as int == SizeOfV(val)
 {
-    match val
-        case VUint64(_)     => size := 8;
-        case VArray(a)      => var v := ComputeSeqSum(a);
-                               if v == 0 {
-                                   size := 8;
-                               } else {
-                                   size := 8 + v;
-                               }
-        case VTuple(t)      => size := ComputeSeqSum(t);
-        case VByteArray(b)  => size := 8 + uint64(|b|);
-        case VCase(c, v)    => var vs := ComputeSizeOf(v);
-                               size := 8 + vs;
+  match val
+    case VUint64(_)     => size := 8;
+    case VArray(a)      => var v := ComputeSeqSum(a);
+                           if v == 0 {
+                             size := 8;
+                           } else {
+                             size := 8 + v;
+                           }
+    case VTuple(t)      => size := ComputeSeqSum(t);
+    case VByteArray(b)  => size := 8 + (|b| as uint64);
+    case VCase(c, v)    => var vs := ComputeSizeOf(v);
+                           size := 8 + vs;
 }
 
 method MarshallUint64(n:uint64, data:array<byte>, index:uint64)
-    requires data != null;
-    requires int(index) + int(Uint64Size()) <= data.Length;
-    requires 0 <= int(index) + int(Uint64Size()) < 0x1_0000_0000_0000_0000;  // Needed to prevent overflow below
-    requires data.Length < 0x1_0000_0000_0000_0000;
-    modifies data;
-    ensures  SeqByteToUint64(data[index..index+uint64(Uint64Size())]) == n;
-    ensures  !parse_Uint64(data[index .. index+uint64(Uint64Size())]).0.None?;
-    ensures  !parse_Uint64(data[index .. ]).0.None?;
-    ensures  var tuple := parse_Uint64(data[index .. index+uint64(Uint64Size())]);
-             tuple.0.v.u == n && tuple.1 == [];
-    ensures  var tuple := parse_Uint64(data[index .. ]);
-             tuple.0.v.u == n && tuple.1 == data[index+uint64(Uint64Size())..];
-    ensures  data[0..index] == old(data[0..index]);
-    ensures  data[index+uint64(Uint64Size())..] == old(data[index+uint64(Uint64Size())..]);
-    ensures  forall i :: 0 <= i < index ==> data[i] == old(data[i]);
-    ensures  forall i :: int(index) + int(Uint64Size()) <= i < data.Length ==> data[i] == old(data[i]);
+  requires (index as int) + (Uint64Size() as int) <= data.Length
+  requires 0 <= (index as int) + (Uint64Size() as int) < 0x1_0000_0000_0000_0000  // Needed to prevent overflow below
+  requires data.Length < 0x1_0000_0000_0000_0000
+  modifies data
+  ensures  SeqByteToUint64(data[index..index+Uint64Size()]) == n
+  ensures  !parse_Uint64(data[index .. index+Uint64Size()]).0.None?
+  ensures  !parse_Uint64(data[index .. ]).0.None?
+  ensures  var tuple := parse_Uint64(data[index .. index+Uint64Size()]);
+           tuple.0.v.u == n && tuple.1 == []
+  ensures  var tuple := parse_Uint64(data[index .. ]);
+           tuple.0.v.u == n && tuple.1 == data[index+Uint64Size()..]
+  ensures  data[0..index] == old(data[0..index])
+  ensures  data[index+Uint64Size()..] == old(data[index+Uint64Size()..])
+  ensures  forall i :: 0 <= i < index ==> data[i] == old(data[i])
+  ensures  forall i :: (index as int) + (Uint64Size() as int) <= i < data.Length ==> data[i] == old(data[i])
 {
-    var tuple := parse_Uint64(data[index .. ]);
-    MarshallUint64_guts(n, data, index);
+  MarshallUint64_guts(n, data, index);
+  var tuple := parse_Uint64(data[index .. ]);
 }
 
 lemma lemma_marshall_array_contents(contents:seq<V>, eltType:G, marshalled_bytes:seq<byte>, trace:seq<seq<byte>>)
-    requires forall v :: v in contents ==> ValInGrammar(v, eltType);
-    requires forall v :: v in contents ==> ValidVal(v);
-    requires ValidGrammar(eltType);
-    requires |marshalled_bytes| < 0x1_0000_0000_0000_0000;
-    requires |contents| < 0x1_0000_0000_0000_0000;
-    requires |contents| == |trace|;
-    requires |marshalled_bytes| == SeqSum(contents);
-    requires marshalled_bytes == SeqCatRev(trace);
-    requires forall j :: 0 <= j < |trace| ==> SizeOfV(contents[j]) == |trace[j]| < 0x1_0000_0000_0000_0000;
-    requires forall j :: 0 <= j < |trace| ==> var (val, rest) := parse_Val(trace[j], eltType); val.Some? && val.v == contents[j]; 
-
-    ensures  parse_Array_contents(marshalled_bytes, eltType, uint64(|contents|)).0.Some?;
-    ensures  parse_Array_contents(marshalled_bytes, eltType, uint64(|contents|)).0.v == contents;
+  requires forall v :: v in contents ==> ValInGrammar(v, eltType)
+  requires forall v :: v in contents ==> ValidVal(v)
+  requires ValidGrammar(eltType)
+  requires |marshalled_bytes| < 0x1_0000_0000_0000_0000
+  requires |contents| < 0x1_0000_0000_0000_0000
+  requires |contents| == |trace|
+  requires |marshalled_bytes| == SeqSum(contents)
+  requires marshalled_bytes == SeqCatRev(trace)
+  requires forall j :: 0 <= j < |trace| ==> SizeOfV(contents[j]) == |trace[j]| < 0x1_0000_0000_0000_0000
+  requires forall j :: 0 <= j < |trace| ==> var (val, rest) := parse_Val(trace[j], eltType); val.Some? && val.v == contents[j];
+  ensures  parse_Array_contents(marshalled_bytes, eltType, |contents| as uint64).0.Some?
+  ensures  parse_Array_contents(marshalled_bytes, eltType, |contents| as uint64).0.v == contents
 {
-    if |contents| == 0 {
-        reveal_parse_Array_contents();
-    } else {
-        var val_tuple := parse_Val(marshalled_bytes, eltType);
-        var val, rest1 := val_tuple.0, val_tuple.1;
-        var rest_tuple := parse_Array_contents(rest1, eltType, uint64(|contents|)-1);
-        var others, rest2 := rest_tuple.0, rest_tuple.1;
-        var target := parse_Array_contents(marshalled_bytes, eltType, uint64(|contents|)).0;
-        calc {
-            target;
-                { reveal_parse_Array_contents(); }
-            if !val.None? && !others.None? then Some([val.v] + others.v) else None;
-        }
-
-        calc {
-            SeqCatRev(trace);
-                { lemma_SeqCat_equivalent(trace); }
-            SeqCat(trace);
-        }
-
-        assert marshalled_bytes[0..SizeOfV(contents[0])] == trace[0];
-        assert parse_Val(trace[0], eltType).0.Some?;
-        assert parse_Val(trace[0], eltType).0.v == contents[0];
-        lemma_parse_Val_view_specific(marshalled_bytes, contents[0], eltType, 0, |marshalled_bytes|);
-        assert parse_Val(marshalled_bytes[0..|marshalled_bytes|], eltType).0 == Some(contents[0]);
-        assert marshalled_bytes[0..|marshalled_bytes|] == marshalled_bytes;     // OBSERVE
-        assert val.Some? && val.v == contents[0];
-        assert rest1 == marshalled_bytes[SizeOfV(contents[0])..];
-
-        // Prove a requires for the recursive call
-        calc {
-            marshalled_bytes[SizeOfV(contents[0])..];
-                calc {
-                    marshalled_bytes;
-                    SeqCatRev(trace);
-                        { lemma_SeqCat_equivalent(trace); }
-                    SeqCat(trace);
-                    trace[0] + SeqCat(trace[1..]);
-                        { lemma_SeqCat_equivalent(trace[1..]); }
-                    trace[0] + SeqCatRev(trace[1..]);
-                }
-            (trace[0] + SeqCatRev(trace[1..]))[SizeOfV(contents[0])..];
-                { assert |trace[0]| == SizeOfV(contents[0]); }
-            SeqCatRev(trace[1..]);
-        }
-
-        // Prove a requires for the recursive call
-        calc {
-            SeqSum(contents);
-                { reveal_SeqSum(); }
-            SizeOfV(contents[0]) + SeqSum(contents[1..]);
-        }
-        lemma_marshall_array_contents(contents[1..], eltType, marshalled_bytes[SizeOfV(contents[0])..], trace[1..]);
-        assert others.Some?;
-        assert others.v == contents[1..];
-        assert contents == [contents[0]] + contents[1..];
-       
+  if |contents| == 0 {
+    reveal parse_Array_contents();
+  } else {
+    var val_tuple := parse_Val(marshalled_bytes, eltType);
+    var val, rest1 := val_tuple.0, val_tuple.1;
+    var rest_tuple := parse_Array_contents(rest1, eltType, |contents| as uint64-1);
+    var others, rest2 := rest_tuple.0, rest_tuple.1;
+    var target := parse_Array_contents(marshalled_bytes, eltType, |contents| as uint64).0;
+    calc {
+      target;
+        { reveal parse_Array_contents(); }
+      if !val.None? && !others.None? then Some([val.v] + others.v) else None;
     }
+
+    calc {
+      SeqCatRev(trace);
+        { lemma_SeqCat_equivalent(trace); }
+      SeqCat(trace);
+    }
+
+    assert marshalled_bytes[0..SizeOfV(contents[0])] == trace[0];
+    assert parse_Val(trace[0], eltType).0.Some?;
+    assert parse_Val(trace[0], eltType).0.v == contents[0];
+    lemma_parse_Val_view_specific(marshalled_bytes, contents[0], eltType, 0, |marshalled_bytes|);
+    assert parse_Val(marshalled_bytes[0..|marshalled_bytes|], eltType).0 == Some(contents[0]);
+    assert marshalled_bytes[0..|marshalled_bytes|] == marshalled_bytes;     // OBSERVE
+    assert val.Some? && val.v == contents[0];
+    assert rest1 == marshalled_bytes[SizeOfV(contents[0])..];
+
+    // Prove a requires for the recursive call
+    calc {
+      marshalled_bytes[SizeOfV(contents[0])..];
+      calc {
+        marshalled_bytes;
+        SeqCatRev(trace);
+          { lemma_SeqCat_equivalent(trace); }
+        SeqCat(trace);
+        trace[0] + SeqCat(trace[1..]);
+          { lemma_SeqCat_equivalent(trace[1..]); }
+        trace[0] + SeqCatRev(trace[1..]);
+      }
+      (trace[0] + SeqCatRev(trace[1..]))[SizeOfV(contents[0])..];
+        { assert |trace[0]| == SizeOfV(contents[0]); }
+      SeqCatRev(trace[1..]);
+    }
+
+    // Prove a requires for the recursive call
+    calc {
+      SeqSum(contents);
+        { reveal SeqSum(); }
+      SizeOfV(contents[0]) + SeqSum(contents[1..]);
+    }
+    lemma_marshall_array_contents(contents[1..], eltType, marshalled_bytes[SizeOfV(contents[0])..], trace[1..]);
+    assert others.Some?;
+    assert others.v == contents[1..];
+    assert contents == [contents[0]] + contents[1..];
+  }
 }
 
 method{:timeLimitMultiplier 4} MarshallArrayContents(contents:seq<V>, eltType:G, data:array<byte>, index:uint64) returns (size:uint64)
-    requires data != null;
-    requires forall v :: v in contents ==> ValInGrammar(v, eltType);
-    requires forall v :: v in contents ==> ValidVal(v);
-    requires ValidGrammar(eltType);
-    requires int(index) + SeqSum(contents) <= data.Length;
-    requires 0 <= int(index) + SeqSum(contents) < 0x1_0000_0000_0000_0000;
-    requires data.Length < 0x1_0000_0000_0000_0000;
-    requires |contents| < 0x1_0000_0000_0000_0000;
-    decreases eltType, 1, |contents|;
-    modifies data;
-    ensures  parse_Array_contents(data[index..int(index) + SeqSum(contents)], eltType, uint64(|contents|)).0.Some?;
-    ensures  parse_Array_contents(data[index..int(index) + SeqSum(contents)], eltType, uint64(|contents|)).0.v == contents;
-    ensures  forall i :: 0 <= i < index ==> data[i] == old(data[i]);
-    ensures  forall i :: int(index) + SeqSum(contents) <= i < data.Length ==> data[i] == old(data[i]);
-    ensures  int(size) == SeqSum(contents);
+  requires forall v :: v in contents ==> ValInGrammar(v, eltType)
+  requires forall v :: v in contents ==> ValidVal(v)
+  requires ValidGrammar(eltType)
+  requires (index as int) + SeqSum(contents) <= data.Length
+  requires 0 <= (index as int) + SeqSum(contents) < 0x1_0000_0000_0000_0000
+  requires data.Length < 0x1_0000_0000_0000_0000
+  requires |contents| < 0x1_0000_0000_0000_0000
+  decreases eltType, 1, |contents|
+  modifies data
+  ensures  parse_Array_contents(data[index..(index as int) + SeqSum(contents)], eltType, |contents| as uint64).0.Some?
+  ensures  parse_Array_contents(data[index..(index as int) + SeqSum(contents)], eltType, |contents| as uint64).0.v == contents
+  ensures  forall i :: 0 <= i < index ==> data[i] == old(data[i])
+  ensures  forall i :: (index as int) + SeqSum(contents) <= i < data.Length ==> data[i] == old(data[i])
+  ensures  size as int == SeqSum(contents)
 {
-    var i:uint64 := 0;
-    var cur_index := index;
-    reveal_SeqSum();
-    reveal_parse_Array_contents();
+  var i:int := 0;
+  var cur_index := index;
+  reveal SeqSum();
+  reveal parse_Array_contents();
 
-    ghost var trace := [];
-    ghost var marshalled_bytes := [];
+  ghost var trace := [];
+  ghost var marshalled_bytes := [];
 
-    while i < uint64(|contents|)
-        invariant 0 <= int(i) <= |contents|;
-        invariant 0 <= int(index) <= int(index) + SeqSum(contents[..i]) <= data.Length;
-        invariant int(cur_index) == int(index) + SeqSum(contents[..i]);
-        invariant forall j :: 0 <= j < index ==> data[j] == old(data[j]);
-        invariant forall j :: int(index) + SeqSum(contents) <= j < data.Length ==> data[j] == old(data[j]);
-        invariant marshalled_bytes == data[index..cur_index];
-        invariant marshalled_bytes == SeqCatRev(trace);
-        invariant |trace| == int(i);
-        invariant forall j :: 0 <= j < |trace| ==> SizeOfV(contents[j]) == |trace[j]| < 0x1_0000_0000_0000_0000;
-        invariant forall j :: 0 <= j < |trace| ==> 
-                        var (val, rest) := parse_Val(trace[j], eltType); 
-                        val.Some? && val.v == contents[j]; 
+  while i < |contents|
+    invariant 0 <= i <= |contents|
+    invariant 0 <= index as int <= (index as int) + SeqSum(contents[..i]) <= data.Length
+    invariant cur_index as int == (index as int) + SeqSum(contents[..i])
+    invariant forall j :: 0 <= j < index ==> data[j] == old(data[j])
+    invariant forall j :: (index as int) + SeqSum(contents) <= j < data.Length ==> data[j] == old(data[j])
+    invariant marshalled_bytes == data[index..cur_index]
+    invariant marshalled_bytes == SeqCatRev(trace)
+    invariant |trace| == i
+    invariant forall j :: 0 <= j < |trace| ==> SizeOfV(contents[j]) == |trace[j]| < 0x1_0000_0000_0000_0000
+    invariant forall j :: 0 <= j < |trace| ==> 
+                    var (val, rest) := parse_Val(trace[j], eltType); 
+                    val.Some? && val.v == contents[j]
+  {
+    lemma_SeqSum_bound(contents, 0x1_0000_0000_0000_0000);
+
+    // Prove we meet MarshallVal's length requirement
+    calc <= {
+      (cur_index as int) + SizeOfV(contents[i]);
+      (index as int) + SeqSum(contents[..i]) + SizeOfV(contents[i]);
+        { lemma_SeqSum_prefix(contents[..i], contents[i]); 
+          assert contents[..i] + [contents[i]] == contents[..i+1]; }
+      (index as int) + SeqSum(contents[..i+1]);
+        { lemma_SeqSum_bound_prefix(contents, contents[..i+1], i+1); }
+      //{ lemma_SeqSum_bound(contents, data.Length - (index as int) + 1); }
+      (index as int) + SeqSum(contents);
+      //data.Length;
+    }
+    var item_size := MarshallVal(contents[i], eltType, data, cur_index);
+    //var item_size := ComputeSizeOf(contents[uint64(i)]);
+
+    ghost var fresh_bytes := data[cur_index..cur_index + item_size];
+    marshalled_bytes := marshalled_bytes + fresh_bytes;
+    forall ensures var (val, rest) := parse_Val(fresh_bytes, eltType);
+                   val.Some? && val.v == contents[i]
     {
-        lemma_SeqSum_bound(contents, 0x1_0000_0000_0000_0000);
-
-        // Prove we meet MarshallVal's length requirement
-        calc <= {
-            int(cur_index) + SizeOfV(contents[i]);
-            int(index) + SeqSum(contents[..i]) + SizeOfV(contents[i]);
-                { lemma_SeqSum_prefix(contents[..i], contents[i]); 
-                  assert contents[..i] + [contents[i]] == contents[..i+1]; }
-            int(index) + SeqSum(contents[..i+1]);
-                { lemma_SeqSum_bound_prefix(contents, contents[..i+1], int(i)+1); }
-                //{ lemma_SeqSum_bound(contents, data.Length - int(index) + 1); }
-            int(index) + SeqSum(contents);
-            //data.Length;
-        }
-        var item_size := MarshallVal(contents[i], eltType, data, cur_index);
-        //var item_size := ComputeSizeOf(contents[uint64(i)]);
-
-        ghost var fresh_bytes := data[cur_index..cur_index + item_size];
-        marshalled_bytes := marshalled_bytes + fresh_bytes;
-        forall () 
-            ensures var (val, rest) := parse_Val(fresh_bytes, eltType);
-                    val.Some? && val.v == contents[i];
-        {
-            assert SizeOfV(contents[i]) <= |fresh_bytes|;  // OBSERVE
-            lemma_parse_Val_view(fresh_bytes, contents[i], eltType, 0);
-        }
-
-        ghost var old_trace := trace;
-        trace := trace + [fresh_bytes];
-
-        ghost var old_cur_index := cur_index;
-        cur_index := cur_index + item_size;
-        i := i + 1;
-
-        // Prove the invariant that we stay within bounds
-        calc <= {
-            int(index) + SeqSum(contents[..i]);
-            calc {
-                SeqSum(contents[..i]);
-                <=  { lemma_SeqSum_bound_prefix(contents, contents[..i], int(i)); }
-                SeqSum(contents);
-            }
-            int(index) + SeqSum(contents);
-            data.Length;
-        }
-        assert {:split_here} true;
-        assert marshalled_bytes == data[index..cur_index];
-
-        // Prove the invariant about our index tracking correctly
-        calc {
-            int(cur_index);
-            int(old_cur_index) + SizeOfV(contents[i-1]);
-            int(index) + SeqSum(contents[..i-1]) + SizeOfV(contents[i-1]);
-                { lemma_SeqSum_prefix(contents[..i-1], contents[i-1]); 
-                  assert contents[..i-1] + [contents[i-1]] == contents[..i]; }
-            int(index) + SeqSum(contents[..i]);
-        }
-        assert int(cur_index) == int(index) + SeqSum(contents[..i]);
-        assert marshalled_bytes == data[index..cur_index];
+      assert SizeOfV(contents[i]) <= |fresh_bytes|;  // OBSERVE
+      lemma_parse_Val_view(fresh_bytes, contents[i], eltType, 0);
     }
 
-    // Prove that parsing will produce the correct result
+    ghost var old_trace := trace;
+    trace := trace + [fresh_bytes];
 
-    // After the while loop, we know:
-    assert contents[..i] == contents;   // OBSERVE
-    assert int(cur_index) == int(index) + SeqSum(contents);
-    assert marshalled_bytes == data[index..int(index)+SeqSum(contents)];
-    //assert marshalled_bytes == SeqCatRev(trace);
-    //assert |trace| == |contents|;
-    lemma_marshall_array_contents(contents, eltType, marshalled_bytes, trace);
-    size := cur_index - index;
+    ghost var old_cur_index := cur_index;
+    cur_index := cur_index + item_size;
+    i := i + 1;
+
+    // Prove the invariant that we stay within bounds
+    calc <= {
+      (index as int) + SeqSum(contents[..i]);
+      calc {
+        SeqSum(contents[..i]);
+        <=  { lemma_SeqSum_bound_prefix(contents, contents[..i], i); }
+        SeqSum(contents);
+      }
+      (index as int) + SeqSum(contents);
+      data.Length;
+    }
+    assert {:split_here} true;
+    assert marshalled_bytes == data[index..cur_index];
+
+    // Prove the invariant about our index tracking correctly
+    calc {
+      cur_index as int;
+      (old_cur_index as int) + SizeOfV(contents[i-1]);
+      (index as int) + SeqSum(contents[..i-1]) + SizeOfV(contents[i-1]);
+        { lemma_SeqSum_prefix(contents[..i-1], contents[i-1]); 
+          assert contents[..i-1] + [contents[i-1]] == contents[..i]; }
+      (index as int) + SeqSum(contents[..i]);
+    }
+    assert cur_index as int == (index as int) + SeqSum(contents[..i]);
+    assert marshalled_bytes == data[index..cur_index];
+  }
+
+  // Prove that parsing will produce the correct result
+
+  // After the while loop, we know:
+  assert contents[..i] == contents;   // OBSERVE
+  assert cur_index as int == (index as int) + SeqSum(contents);
+  assert marshalled_bytes == data[index..(index as int)+SeqSum(contents)];
+  //assert marshalled_bytes == SeqCatRev(trace);
+  //assert |trace| == |contents|;
+  lemma_marshall_array_contents(contents, eltType, marshalled_bytes, trace);
+  size := cur_index - index;
 }
 
 method MarshallArray(val:V, grammar:G, data:array<byte>, index:uint64) returns (size:uint64)
-    requires data != null;
-    requires val.VArray?;
-    requires ValInGrammar(val, grammar);
-    requires ValidGrammar(grammar);
-    requires ValidVal(val);
-    requires int(index) + SizeOfV(val) <= data.Length;
-    requires 0 <= int(index) + SizeOfV(val) < 0x1_0000_0000_0000_0000;  // Needed to prevent overflow below
-    requires data.Length < 0x1_0000_0000_0000_0000;
-    modifies data;
-    decreases grammar, -1;
-    ensures  parse_Val(data[index..int(index) + SizeOfV(val)], grammar).0.Some? &&
-             parse_Val(data[index..int(index) + SizeOfV(val)], grammar).0.v == val;
-    ensures  forall i :: 0 <= i < index ==> data[i] == old(data[i]);
-    ensures  forall i :: int(index) + SizeOfV(val) <= i < data.Length ==> data[i] == old(data[i]);
-    ensures  int(size) == SizeOfV(val);
+  requires val.VArray?
+  requires ValInGrammar(val, grammar)
+  requires ValidGrammar(grammar)
+  requires ValidVal(val)
+  requires (index as int) + SizeOfV(val) <= data.Length
+  requires 0 <= (index as int) + SizeOfV(val) < 0x1_0000_0000_0000_0000   // Needed to prevent overflow below
+  requires data.Length < 0x1_0000_0000_0000_0000
+  modifies data
+  decreases grammar, -1
+  ensures  parse_Val(data[index..(index as int) + SizeOfV(val)], grammar).0.Some? &&
+           parse_Val(data[index..(index as int) + SizeOfV(val)], grammar).0.v == val
+  ensures  forall i :: 0 <= i < index ==> data[i] == old(data[i])
+  ensures  forall i :: (index as int) + SizeOfV(val) <= i < data.Length ==> data[i] == old(data[i])
+  ensures  (size as int) == SizeOfV(val)
 {
-    //assert{:split_here} true;
-    reveal_parse_Val();
-    MarshallUint64(uint64(|val.a|), data, index);
+  //assert{:split_here} true;
+  reveal parse_Val();
+  MarshallUint64(|val.a| as uint64, data, index);
 
-    ghost var tuple := parse_Uint64(data[index..int(index) + SizeOfV(val)]);
-    ghost var len := tuple.0;
-    ghost var rest := tuple.1;
-    assert !len.None?;
-    var contents_size := MarshallArrayContents(val.a, grammar.elt, data, index + Uint64Size());
-    tuple := parse_Uint64(data[index..int(index) + SizeOfV(val)]);
-    assert {:split_here} true;
-    len := tuple.0;
-    rest := tuple.1;
-    assert !len.None?;
-    ghost var contents_tuple := parse_Array_contents(rest, grammar.elt, len.v.u);
-    ghost var contents  := contents_tuple.0;
-    ghost var remainder := contents_tuple.1;
-    assert !contents.None?;
-    size := 8 + contents_size;
+  ghost var tuple := parse_Uint64(data[index..(index as int) + SizeOfV(val)]);
+  ghost var len := tuple.0;
+  ghost var rest := tuple.1;
+  assert !len.None?;
+  var contents_size := MarshallArrayContents(val.a, grammar.elt, data, index + Uint64Size());
+  tuple := parse_Uint64(data[index..(index as int) + SizeOfV(val)]);
+  assert {:split_here} true;
+  len := tuple.0;
+  rest := tuple.1;
+  assert !len.None?;
+  ghost var contents_tuple := parse_Array_contents(rest, grammar.elt, len.v.u);
+  ghost var contents  := contents_tuple.0;
+  ghost var remainder := contents_tuple.1;
+  assert !contents.None?;
+  size := 8 + contents_size;
 }
 
 lemma lemma_marshall_tuple_contents(contents:seq<V>, eltTypes:seq<G>, marshalled_bytes:seq<byte>, trace:seq<seq<byte>>)
-    requires |contents| == |eltTypes|;
-    requires forall i :: 0 <= i < |contents| ==> ValInGrammar(contents[i], eltTypes[i]);
-    requires forall g :: g in eltTypes ==> ValidGrammar(g);
-    requires |eltTypes| < 0x1_0000_0000_0000_0000;
-    requires forall i :: 0 <= i < |contents| ==> ValidVal(contents[i]);
-    requires |marshalled_bytes| < 0x1_0000_0000_0000_0000;
-    requires |contents| < 0x1_0000_0000_0000_0000;
-    requires |contents| == |trace|;
-    requires |marshalled_bytes| == SeqSum(contents);
-    requires marshalled_bytes == SeqCatRev(trace);
-    requires forall j :: 0 <= j < |trace| ==> SizeOfV(contents[j]) == |trace[j]| < 0x1_0000_0000_0000_0000;
-    requires forall j :: 0 <= j < |trace| ==> var (val, rest) := parse_Val(trace[j], eltTypes[j]); val.Some? && val.v == contents[j]; 
-
-    ensures  parse_Tuple_contents(marshalled_bytes, eltTypes).0.Some?;
-    ensures  parse_Tuple_contents(marshalled_bytes, eltTypes).0.v == contents;
+  requires |contents| == |eltTypes|
+  requires forall i :: 0 <= i < |contents| ==> ValInGrammar(contents[i], eltTypes[i])
+  requires forall g :: g in eltTypes ==> ValidGrammar(g)
+  requires |eltTypes| < 0x1_0000_0000_0000_0000
+  requires forall i :: 0 <= i < |contents| ==> ValidVal(contents[i])
+  requires |marshalled_bytes| < 0x1_0000_0000_0000_0000
+  requires |contents| < 0x1_0000_0000_0000_0000
+  requires |contents| == |trace|
+  requires |marshalled_bytes| == SeqSum(contents)
+  requires marshalled_bytes == SeqCatRev(trace)
+  requires forall j :: 0 <= j < |trace| ==> SizeOfV(contents[j]) == |trace[j]| < 0x1_0000_0000_0000_0000
+  requires forall j :: 0 <= j < |trace| ==> var (val, rest) := parse_Val(trace[j], eltTypes[j]); val.Some? && val.v == contents[j];
+  ensures  parse_Tuple_contents(marshalled_bytes, eltTypes).0.Some?
+    ensures  parse_Tuple_contents(marshalled_bytes, eltTypes).0.v == contents
 {
-    if |contents| == 0 {
-        reveal_parse_Tuple_contents();
-    } else {
-        var val_tuple := parse_Val(marshalled_bytes, eltTypes[0]);
-        var val, rest1 := val_tuple.0, val_tuple.1;
-        var rest_tuple := parse_Tuple_contents(rest1, eltTypes[1..]);
-        var others, rest2 := rest_tuple.0, rest_tuple.1;
-        var target := parse_Tuple_contents(marshalled_bytes, eltTypes).0;
-        calc {
-            target;
-                { reveal_parse_Tuple_contents(); }
-            if !val.None? && !others.None? then Some([val.v] + others.v) else None;
-        }
-
-        calc {
-            SeqCatRev(trace);
-                { lemma_SeqCat_equivalent(trace); }
-            SeqCat(trace);
-        }
-
-        assert marshalled_bytes[0..SizeOfV(contents[0])] == trace[0];
-        assert parse_Val(trace[0], eltTypes[0]).0.Some?;
-        assert parse_Val(trace[0], eltTypes[0]).0.v == contents[0];
-        lemma_parse_Val_view_specific(marshalled_bytes, contents[0], eltTypes[0], 0, |marshalled_bytes|);
-        assert parse_Val(marshalled_bytes[0..|marshalled_bytes|], eltTypes[0]).0 == Some(contents[0]);
-        assert marshalled_bytes[0..|marshalled_bytes|] == marshalled_bytes;     // OBSERVE
-        assert val.Some? && val.v == contents[0];
-        assert rest1 == marshalled_bytes[SizeOfV(contents[0])..];
-
-        // Prove a requires for the recursive call
-        calc {
-            marshalled_bytes[SizeOfV(contents[0])..];
-                calc {
-                    marshalled_bytes;
-                    SeqCatRev(trace);
-                        { lemma_SeqCat_equivalent(trace); }
-                    SeqCat(trace);
-                    trace[0] + SeqCat(trace[1..]);
-                        { lemma_SeqCat_equivalent(trace[1..]); }
-                    trace[0] + SeqCatRev(trace[1..]);
-                }
-            (trace[0] + SeqCatRev(trace[1..]))[SizeOfV(contents[0])..];
-                { assert |trace[0]| == SizeOfV(contents[0]); }
-            SeqCatRev(trace[1..]);
-        }
-
-        // Prove a requires for the recursive call
-        calc {
-            SeqSum(contents);
-                { reveal_SeqSum(); }
-            SizeOfV(contents[0]) + SeqSum(contents[1..]);
-        }
-        lemma_marshall_tuple_contents(contents[1..], eltTypes[1..], marshalled_bytes[SizeOfV(contents[0])..], trace[1..]);
-        assert others.Some?;
-        assert others.v == contents[1..];
-        assert contents == [contents[0]] + contents[1..];
-       
+  if |contents| == 0 {
+    reveal parse_Tuple_contents();
+  } else {
+    var val_tuple := parse_Val(marshalled_bytes, eltTypes[0]);
+    var val, rest1 := val_tuple.0, val_tuple.1;
+    var rest_tuple := parse_Tuple_contents(rest1, eltTypes[1..]);
+    var others, rest2 := rest_tuple.0, rest_tuple.1;
+    var target := parse_Tuple_contents(marshalled_bytes, eltTypes).0;
+    calc {
+      target;
+        { reveal parse_Tuple_contents(); }
+      if !val.None? && !others.None? then Some([val.v] + others.v) else None;
     }
+
+    calc {
+      SeqCatRev(trace);
+        { lemma_SeqCat_equivalent(trace); }
+      SeqCat(trace);
+    }
+
+    assert marshalled_bytes[0..SizeOfV(contents[0])] == trace[0];
+    assert parse_Val(trace[0], eltTypes[0]).0.Some?;
+    assert parse_Val(trace[0], eltTypes[0]).0.v == contents[0];
+    lemma_parse_Val_view_specific(marshalled_bytes, contents[0], eltTypes[0], 0, |marshalled_bytes|);
+    assert parse_Val(marshalled_bytes[0..|marshalled_bytes|], eltTypes[0]).0 == Some(contents[0]);
+    assert marshalled_bytes[0..|marshalled_bytes|] == marshalled_bytes;     // OBSERVE
+    assert val.Some? && val.v == contents[0];
+    assert rest1 == marshalled_bytes[SizeOfV(contents[0])..];
+
+    // Prove a requires for the recursive call
+    calc {
+      marshalled_bytes[SizeOfV(contents[0])..];
+      calc {
+        marshalled_bytes;
+        SeqCatRev(trace);
+          { lemma_SeqCat_equivalent(trace); }
+        SeqCat(trace);
+        trace[0] + SeqCat(trace[1..]);
+          { lemma_SeqCat_equivalent(trace[1..]); }
+        trace[0] + SeqCatRev(trace[1..]);
+      }
+      (trace[0] + SeqCatRev(trace[1..]))[SizeOfV(contents[0])..];
+        { assert |trace[0]| == SizeOfV(contents[0]); }
+      SeqCatRev(trace[1..]);
+    }
+
+    // Prove a requires for the recursive call
+    calc {
+      SeqSum(contents);
+        { reveal SeqSum(); }
+      SizeOfV(contents[0]) + SeqSum(contents[1..]);
+    }
+    lemma_marshall_tuple_contents(contents[1..], eltTypes[1..], marshalled_bytes[SizeOfV(contents[0])..], trace[1..]);
+    assert others.Some?;
+    assert others.v == contents[1..];
+    assert contents == [contents[0]] + contents[1..];
+  }
 }
 
 method{:timeLimitMultiplier 2} MarshallTupleContents(contents:seq<V>, eltTypes:seq<G>, data:array<byte>, index:uint64) returns (size:uint64)
-    requires data != null;
-    requires |contents| == |eltTypes|;
-    requires forall i :: 0 <= i < |contents| ==> ValInGrammar(contents[i], eltTypes[i]);
-    requires forall g :: g in eltTypes ==> ValidGrammar(g);
-    requires |eltTypes| < 0x1_0000_0000_0000_0000;
-    requires forall i :: 0 <= i < |contents| ==> ValidVal(contents[i]);
-    requires int(index) + SeqSum(contents) <= data.Length;
-    requires 0 <= int(index) + SeqSum(contents) < 0x1_0000_0000_0000_0000;
-    requires data.Length < 0x1_0000_0000_0000_0000;
-    requires |contents| < 0x1_0000_0000_0000_0000;
-    decreases eltTypes, 1, |contents|;
-    modifies data;
-    ensures  parse_Tuple_contents(data[index..int(index) + SeqSum(contents)], eltTypes).0.Some?;
-    ensures  parse_Tuple_contents(data[index..int(index) + SeqSum(contents)], eltTypes).0.v == contents;
-    ensures  forall i :: 0 <= i < index ==> data[i] == old(data[i]);
-    ensures  forall i :: int(index) + SeqSum(contents) <= i < data.Length ==> data[i] == old(data[i]);
-    ensures  int(size) == SeqSum(contents);
+  requires |contents| == |eltTypes|
+  requires forall i :: 0 <= i < |contents| ==> ValInGrammar(contents[i], eltTypes[i])
+  requires forall g :: g in eltTypes ==> ValidGrammar(g)
+  requires |eltTypes| < 0x1_0000_0000_0000_0000
+  requires forall i :: 0 <= i < |contents| ==> ValidVal(contents[i])
+  requires (index as int) + SeqSum(contents) <= data.Length
+  requires 0 <= (index as int) + SeqSum(contents) < 0x1_0000_0000_0000_0000
+  requires data.Length < 0x1_0000_0000_0000_0000
+  requires |contents| < 0x1_0000_0000_0000_0000
+  decreases eltTypes, 1, |contents|
+  modifies data
+  ensures  parse_Tuple_contents(data[index..(index as int) + SeqSum(contents)], eltTypes).0.Some?
+  ensures  parse_Tuple_contents(data[index..(index as int) + SeqSum(contents)], eltTypes).0.v == contents
+  ensures  forall i :: 0 <= i < index ==> data[i] == old(data[i])
+  ensures  forall i :: (index as int) + SeqSum(contents) <= i < data.Length ==> data[i] == old(data[i])
+  ensures  size as int == SeqSum(contents)
 {
-    var i:uint64 := 0;
-    var cur_index := index;
-    reveal_SeqSum();
-    reveal_parse_Tuple_contents();
+  var i:int := 0;
+  var cur_index := index;
+  reveal SeqSum();
+  reveal parse_Tuple_contents();
 
-    ghost var trace := [];
-    ghost var marshalled_bytes := [];
+  ghost var trace := [];
+  ghost var marshalled_bytes := [];
 
-    while i < uint64(|contents|)
-        invariant 0 <= int(i) <= |contents|;
-        invariant 0 <= int(index) <= int(index) + SeqSum(contents[..i]) <= data.Length;
-        invariant int(cur_index) == int(index) + SeqSum(contents[..i]);
-        invariant forall j :: 0 <= j < index ==> data[j] == old(data[j]);
-        invariant forall j :: int(index) + SeqSum(contents) <= j < data.Length ==> data[j] == old(data[j]);
-        invariant marshalled_bytes == data[index..cur_index];
-        invariant marshalled_bytes == SeqCatRev(trace);
-        invariant |trace| == int(i);
-        invariant forall j :: 0 <= j < |trace| ==> SizeOfV(contents[j]) == |trace[j]| < 0x1_0000_0000_0000_0000;
-        invariant forall j :: 0 <= j < |trace| ==> 
-                        var (val, rest) := parse_Val(trace[j], eltTypes[j]); 
-                        val.Some? && val.v == contents[j]; 
+  while i < |contents|
+    invariant 0 <= i <= |contents|
+    invariant 0 <= index as int <= (index as int) + SeqSum(contents[..i]) <= data.Length
+    invariant cur_index as int == (index as int) + SeqSum(contents[..i])
+    invariant forall j :: 0 <= j < index ==> data[j] == old(data[j])
+    invariant forall j :: (index as int) + SeqSum(contents) <= j < data.Length ==> data[j] == old(data[j])
+    invariant marshalled_bytes == data[index..cur_index]
+    invariant marshalled_bytes == SeqCatRev(trace)
+    invariant |trace| == i
+    invariant forall j :: 0 <= j < |trace| ==> SizeOfV(contents[j]) == |trace[j]| < 0x1_0000_0000_0000_0000
+    invariant forall j :: 0 <= j < |trace| ==> 
+                    var (val, rest) := parse_Val(trace[j], eltTypes[j]); 
+                    val.Some? && val.v == contents[j]
+  {
+    lemma_SeqSum_bound(contents, 0x1_0000_0000_0000_0000);
+    ghost var old_marshalled_bytes := marshalled_bytes;
+    ghost var old_data := data[index..cur_index];
+    assert old_marshalled_bytes == old_data;
+
+    // Prove we meet MarshallVal's length requirement
+    calc <= {
+      (cur_index as int) + SizeOfV(contents[i]);
+      (index as int) + SeqSum(contents[..i]) + SizeOfV(contents[i]);
+        { lemma_SeqSum_prefix(contents[..i], contents[i]); 
+          assert contents[..i] + [contents[i]] == contents[..i+1]; }
+      (index as int) + SeqSum(contents[..i+1]);
+        { lemma_SeqSum_bound_prefix(contents, contents[..i+1], i+1); }
+      //{ lemma_SeqSum_bound(contents, data.Length - (index as int) + 1); }
+      (index as int) + SeqSum(contents);
+      //data.Length;
+    }
+    var item_size := MarshallVal(contents[i], eltTypes[i], data, cur_index);
+    //var item_size := ComputeSizeOf(contents[i]);
+
+    ghost var fresh_bytes := data[cur_index..cur_index + item_size];
+    marshalled_bytes := marshalled_bytes + fresh_bytes;
+    forall ensures var (val, rest) := parse_Val(fresh_bytes, eltTypes[i]);
+                   val.Some? && val.v == contents[i];
     {
-        lemma_SeqSum_bound(contents, 0x1_0000_0000_0000_0000);
-        ghost var old_marshalled_bytes := marshalled_bytes;
-        ghost var old_data := data[index..cur_index];
-        assert old_marshalled_bytes == old_data;
-
-        // Prove we meet MarshallVal's length requirement
-        calc <= {
-            int(cur_index) + SizeOfV(contents[i]);
-            int(index) + SeqSum(contents[..i]) + SizeOfV(contents[i]);
-                { lemma_SeqSum_prefix(contents[..i], contents[i]); 
-                  assert contents[..i] + [contents[i]] == contents[..i+1]; }
-            int(index) + SeqSum(contents[..i+1]);
-                { lemma_SeqSum_bound_prefix(contents, contents[..i+1], int(i)+1); }
-                //{ lemma_SeqSum_bound(contents, data.Length - int(index) + 1); }
-            int(index) + SeqSum(contents);
-            //data.Length;
-        }
-        var item_size := MarshallVal(contents[i], eltTypes[i], data, cur_index);
-        //var item_size := ComputeSizeOf(contents[uint64(i)]);
-
-        ghost var fresh_bytes := data[cur_index..cur_index + item_size];
-        marshalled_bytes := marshalled_bytes + fresh_bytes;
-        forall () 
-            ensures var (val, rest) := parse_Val(fresh_bytes, eltTypes[i]);
-                    val.Some? && val.v == contents[i];
-        {
-            assert SizeOfV(contents[i]) <= |fresh_bytes|;  // OBSERVE
-            lemma_parse_Val_view(fresh_bytes, contents[i], eltTypes[i], 0);
-        }
-
-        ghost var old_trace := trace;
-        trace := trace + [fresh_bytes];
-
-        ghost var old_cur_index := cur_index;
-        cur_index := cur_index + item_size;
-        i := i + 1;
-        
-        assert {:split_here} true;
-
-        // Prove the invariant about marshalled_bytes' contents
-        calc {
-            marshalled_bytes;
-            old_marshalled_bytes + fresh_bytes;
-            old_data + fresh_bytes;
-            data[index..old_cur_index] + fresh_bytes;
-            data[index..old_cur_index] + data[old_cur_index..cur_index];
-            data[index..cur_index];
-        }
-
-        // Prove the invariant that we stay within bounds
-        calc <= {
-            int(index) + SeqSum(contents[..i]);
-            calc {
-                SeqSum(contents[..i]);
-                <=  { lemma_SeqSum_bound_prefix(contents, contents[..i], int(i)); }
-                SeqSum(contents);
-            }
-            int(index) + SeqSum(contents);
-            data.Length;
-        }
-
-        // Prove the invariant about our index tracking correctly
-        calc {
-            int(cur_index);
-            int(old_cur_index) + SizeOfV(contents[i-1]);
-            int(index) + SeqSum(contents[..i-1]) + SizeOfV(contents[i-1]);
-                { lemma_SeqSum_prefix(contents[..i-1], contents[i-1]); 
-                  assert contents[..i-1] + [contents[i-1]] == contents[..i]; }
-            int(index) + SeqSum(contents[..i]);
-        }
-        assert int(cur_index) == int(index) + SeqSum(contents[..i]);
+      assert SizeOfV(contents[i]) <= |fresh_bytes|;  // OBSERVE
+      lemma_parse_Val_view(fresh_bytes, contents[i], eltTypes[i], 0);
     }
 
-    // Prove that parsing will produce the correct result
+    ghost var old_trace := trace;
+    trace := trace + [fresh_bytes];
 
-    // After the while loop, we know:
-    assert contents[..i] == contents;   // OBSERVE
-    assert int(cur_index) == int(index) + SeqSum(contents);
-    assert marshalled_bytes == data[index..int(index)+SeqSum(contents)];
-    //assert marshalled_bytes == SeqCatRev(trace);
-    //assert |trace| == |contents|;
-    lemma_marshall_tuple_contents(contents, eltTypes, marshalled_bytes, trace);
-    size := cur_index - index;
+    ghost var old_cur_index := cur_index;
+    cur_index := cur_index + item_size;
+    i := i + 1;
+        
+    assert {:split_here} true;
+
+    // Prove the invariant about marshalled_bytes' contents
+    calc {
+      marshalled_bytes;
+      old_marshalled_bytes + fresh_bytes;
+      old_data + fresh_bytes;
+      data[index..old_cur_index] + fresh_bytes;
+      data[index..old_cur_index] + data[old_cur_index..cur_index];
+      data[index..cur_index];
+    }
+
+    // Prove the invariant that we stay within bounds
+    calc <= {
+      (index as int) + SeqSum(contents[..i]);
+      calc {
+        SeqSum(contents[..i]);
+        <=  { lemma_SeqSum_bound_prefix(contents, contents[..i], i); }
+        SeqSum(contents);
+      }
+      (index as int) + SeqSum(contents);
+      data.Length;
+    }
+
+    // Prove the invariant about our index tracking correctly
+    calc {
+      cur_index as int;
+      (old_cur_index as int) + SizeOfV(contents[i-1]);
+      (index as int) + SeqSum(contents[..i-1]) + SizeOfV(contents[i-1]);
+        { lemma_SeqSum_prefix(contents[..i-1], contents[i-1]); 
+          assert contents[..i-1] + [contents[i-1]] == contents[..i]; }
+      (index as int) + SeqSum(contents[..i]);
+    }
+    assert cur_index as int == (index as int) + SeqSum(contents[..i]);
+  }
+
+  // Prove that parsing will produce the correct result
+
+  // After the while loop, we know:
+  assert contents[..i] == contents;   // OBSERVE
+  assert cur_index as int == (index as int) + SeqSum(contents);
+  assert marshalled_bytes == data[index..(index as int)+SeqSum(contents)];
+  //assert marshalled_bytes == SeqCatRev(trace);
+  //assert |trace| == |contents|;
+  lemma_marshall_tuple_contents(contents, eltTypes, marshalled_bytes, trace);
+  size := cur_index - index;
 }
 
 method MarshallTuple(val:V, grammar:G, data:array<byte>, index:uint64) returns (size:uint64)
-    requires data != null;
-    requires val.VTuple?;
-    requires ValidVal(val);
-    requires ValidGrammar(grammar);
-    requires ValInGrammar(val, grammar);
-    requires int(index) + SizeOfV(val) <= data.Length;
-    requires 0 <= int(index) + SizeOfV(val) < 0x1_0000_0000_0000_0000;  // Needed to prevent overflow below
-    requires data.Length < 0x1_0000_0000_0000_0000;
-    modifies data;
-    decreases grammar, -1;
-    ensures  parse_Val(data[index..int(index) + SizeOfV(val)], grammar).0.Some? &&
-             parse_Val(data[index..int(index) + SizeOfV(val)], grammar).0.v == val;
-    ensures  forall i :: 0 <= i < index ==> data[i] == old(data[i]);
-    ensures  forall i :: int(index) + SizeOfV(val) <= i < data.Length ==> data[i] == old(data[i]);
-    ensures  int(size) == SizeOfV(val);
+  requires val.VTuple?
+  requires ValidVal(val)
+  requires ValidGrammar(grammar)
+  requires ValInGrammar(val, grammar)
+  requires (index as int) + SizeOfV(val) <= data.Length
+  requires 0 <= (index as int) + SizeOfV(val) < 0x1_0000_0000_0000_0000   // Needed to prevent overflow below
+  requires data.Length < 0x1_0000_0000_0000_0000
+  modifies data
+  decreases grammar, -1
+  ensures  parse_Val(data[index..(index as int) + SizeOfV(val)], grammar).0.Some? &&
+           parse_Val(data[index..(index as int) + SizeOfV(val)], grammar).0.v == val
+  ensures  forall i :: 0 <= i < index ==> data[i] == old(data[i])
+  ensures  forall i :: (index as int) + SizeOfV(val) <= i < data.Length ==> data[i] == old(data[i])
+  ensures  size as int == SizeOfV(val)
 {
-    size := MarshallTupleContents(val.t, grammar.t, data, index);
+  size := MarshallTupleContents(val.t, grammar.t, data, index);
 
-    calc {
-        parse_Val(data[index..int(index) + SizeOfV(val)], grammar);
-            { reveal_parse_Val(); }
-        parse_Tuple(data[index..int(index) + SizeOfV(val)], grammar.t);
-    }
+  calc {
+    parse_Val(data[index..(index as int) + SizeOfV(val)], grammar);
+      { reveal parse_Val(); }
+    parse_Tuple(data[index..(index as int) + SizeOfV(val)], grammar.t);
+  }
 }
 
 method MarshallBytes(bytes:seq<byte>, data:array<byte>, index:uint64)
-    requires data != null;
-    requires int(index) + |bytes| <= data.Length;
-    requires 0 <= int(index) + |bytes| < 0x1_0000_0000_0000_0000;  // Needed to prevent overflow below
-    requires data.Length < 0x1_0000_0000_0000_0000;
-    modifies data;
-    ensures  forall i :: 0 <= i < index ==> data[i] == old(data[i]);
-    ensures  forall i :: int(index) <= i < int(index) + |bytes| ==> data[i] == bytes[i - int(index)];
-    ensures  forall i :: int(index) + |bytes| <= i < data.Length ==> data[i] == old(data[i]);
+  requires (index as int) + |bytes| <= data.Length
+  requires 0 <= (index as int) + |bytes| < 0x1_0000_0000_0000_0000   // Needed to prevent overflow below
+  requires data.Length < 0x1_0000_0000_0000_0000
+  modifies data
+  ensures  forall i :: 0 <= i < index ==> data[i] == old(data[i])
+  ensures  forall i :: (index as int) <= i < (index as int) + |bytes| ==> data[i] == bytes[i - (index as int)]
+  ensures  forall i :: (index as int) + |bytes| <= i < data.Length ==> data[i] == old(data[i])
 {
-    Arrays.CopySeqIntoArray(bytes, 0, data, index, uint64(|bytes|));
+  Arrays.CopySeqIntoArray(bytes, 0, data, index, |bytes| as uint64);
 
-    /*
-    var j:uint64 := 0;
+  /*
+  var j:uint64 := 0;
 
-    while (j < uint64(|bytes|))
-        invariant 0 <= int(j) <= |bytes|;
-        invariant forall i:int :: 0 <= i < int(index) ==> data[i] == old(data[i]);
-        invariant forall i:int :: int(index) <= i < int(index) + int(j) ==> data[i] == bytes[i-int(index)];
-        invariant forall i:int :: int(index) + |bytes| <= i < data.Length ==> data[i] == old(data[i]);
-    {
-        data[index + j] := bytes[j];
-        j := j + 1;
-    }
-    */
+  while (j < uint64(|bytes|))
+    invariant 0 <= j as int <= |bytes|
+    invariant forall i:int :: 0 <= i < (index as int) ==> data[i] == old(data[i])
+    invariant forall i:int :: index as int <= i < (index as int) + (j as int) ==> data[i] == bytes[i-(index as int)]
+    invariant forall i:int :: (index as int) + |bytes| <= i < data.Length ==> data[i] == old(data[i])
+  {
+    data[index + j] := bytes[j];
+    j := j + 1;
+  }
+  */
 }
 
 method MarshallByteArray(val:V, grammar:G, data:array<byte>, index:uint64) returns (size:uint64)
-    requires data != null;
-    requires val.VByteArray?;
-    requires ValidGrammar(grammar);
-    requires ValInGrammar(val, grammar);
-    requires ValidVal(val);
-    requires int(index) + SizeOfV(val) <= data.Length;
-    requires 0 <= int(index) + SizeOfV(val) < 0x1_0000_0000_0000_0000;  // Needed to prevent overflow below
-    requires data.Length < 0x1_0000_0000_0000_0000;
-    modifies data;
-    decreases grammar;
-    ensures  parse_Val(data[index..int(index) + SizeOfV(val)], grammar).0.Some? &&
-             parse_Val(data[index..int(index) + SizeOfV(val)], grammar).0.v == val;
-    ensures  forall i :: 0 <= i < index ==> data[i] == old(data[i]);
-    ensures  forall i :: int(index) + SizeOfV(val) <= i < data.Length ==> data[i] == old(data[i]);
-    ensures  int(size) == SizeOfV(val);
+  requires val.VByteArray?
+  requires ValidGrammar(grammar)
+  requires ValInGrammar(val, grammar)
+  requires ValidVal(val)
+  requires (index as int) + SizeOfV(val) <= data.Length
+  requires 0 <= (index as int) + SizeOfV(val) < 0x1_0000_0000_0000_0000   // Needed to prevent overflow below
+  requires data.Length < 0x1_0000_0000_0000_0000
+  modifies data
+  decreases grammar
+  ensures  parse_Val(data[index..(index as int) + SizeOfV(val)], grammar).0.Some? &&
+           parse_Val(data[index..(index as int) + SizeOfV(val)], grammar).0.v == val
+  ensures  forall i :: 0 <= i < index ==> data[i] == old(data[i]);
+  ensures  forall i :: (index as int) + SizeOfV(val) <= i < data.Length ==> data[i] == old(data[i])
+  ensures  size as int == SizeOfV(val)
 {
-    MarshallUint64(uint64(|val.b|), data, index);
-    assert SeqByteToUint64(data[index..index+uint64(Uint64Size())]) == uint64(|val.b|);
-    MarshallBytes(val.b, data, index + 8);
+  MarshallUint64(|val.b| as uint64, data, index);
+  assert SeqByteToUint64(data[index..index+Uint64Size()]) == (|val.b| as uint64);
+  MarshallBytes(val.b, data, index + 8);
 
-    calc {
-        parse_Val(data[index..int(index) + SizeOfV(val)], grammar);
-            { reveal_parse_Val(); }
-        parse_ByteArray(data[index..int(index) + SizeOfV(val)]);
-    }
-    ghost var data_seq := data[index..int(index) + SizeOfV(val)];
-    ghost var tuple := parse_Uint64(data_seq);
-    ghost var len := tuple.0;
-    ghost var rest := tuple.1;
-    assert{:split_here} true;
-    // assert len.v.u == uint64(|val.b|);
-    
-    assert rest == data[index + 8..int(index) + SizeOfV(val)] == val.b;
-    assert !len.None? && int(len.v.u) <= |rest|;
-    assert rest[0..len.v.u] == val.b;       // OBSERVE
-    size := 8 + uint64(|val.b|);
+  calc {
+    parse_Val(data[index..(index as int) + SizeOfV(val)], grammar);
+      { reveal parse_Val(); }
+    parse_ByteArray(data[index..(index as int) + SizeOfV(val)]);
+  }
+  ghost var data_seq := data[index..(index as int) + SizeOfV(val)];
+  ghost var tuple := parse_Uint64(data_seq);
+  ghost var len := tuple.0;
+  ghost var rest := tuple.1;
+  assert{:split_here} true;
+  // assert len.v.u == uint64(|val.b|);
+  
+  assert rest == data[index + 8..(index as int) + SizeOfV(val)] == val.b;
+  assert !len.None? && (len.v.u as int) <= |rest|;
+  assert rest[0..len.v.u] == val.b;       // OBSERVE
+  size := 8 + (|val.b| as uint64);
 }
 
 method MarshallCase(val:V, grammar:G, data:array<byte>, index:uint64) returns (size:uint64)
-    requires data != null;
-    requires val.VCase?;
-    requires ValidGrammar(grammar);
-    requires ValInGrammar(val, grammar);
-    requires ValidVal(val);
-    requires int(index) + SizeOfV(val) <= data.Length;
-    requires 0 <= int(index) + SizeOfV(val) < 0x1_0000_0000_0000_0000;  // Needed to prevent overflow below
-    requires data.Length < 0x1_0000_0000_0000_0000;
-    modifies data;
-    decreases grammar, -1;
-    ensures  parse_Val(data[index..int(index) + SizeOfV(val)], grammar).0.Some? &&
-             parse_Val(data[index..int(index) + SizeOfV(val)], grammar).0.v == val;
-    ensures  forall i :: 0 <= i < index ==> data[i] == old(data[i]);
-    ensures  forall i :: int(index) + SizeOfV(val) <= i < data.Length ==> data[i] == old(data[i]);
-    ensures  int(size) == SizeOfV(val);
+  requires val.VCase?
+  requires ValidGrammar(grammar)
+  requires ValInGrammar(val, grammar)
+  requires ValidVal(val)
+  requires (index as int) + SizeOfV(val) <= data.Length
+  requires 0 <= (index as int) + SizeOfV(val) < 0x1_0000_0000_0000_0000   // Needed to prevent overflow below
+  requires data.Length < 0x1_0000_0000_0000_0000
+  modifies data
+  decreases grammar, -1
+  ensures  parse_Val(data[index..(index as int) + SizeOfV(val)], grammar).0.Some? &&
+           parse_Val(data[index..(index as int) + SizeOfV(val)], grammar).0.v == val
+  ensures  forall i :: 0 <= i < index ==> data[i] == old(data[i])
+  ensures  forall i :: (index as int) + SizeOfV(val) <= i < data.Length ==> data[i] == old(data[i])
+  ensures  size as int == SizeOfV(val)
 {
-    MarshallUint64(val.c, data, index);
-    ghost var int_bytes := data[index..index+Uint64Size()];
-    ghost var tuple0 := parse_Uint64(int_bytes);
-    ghost var caseID0 := tuple0.0;
-    ghost var rest10   := tuple0.1;
-    assert !caseID0.None?;
-    assert caseID0.v.u == val.c;
+  MarshallUint64(val.c, data, index);
+  ghost var int_bytes := data[index..index+Uint64Size()];
+  ghost var tuple0 := parse_Uint64(int_bytes);
+  ghost var caseID0 := tuple0.0;
+  ghost var rest10   := tuple0.1;
+  assert !caseID0.None?;
+  assert caseID0.v.u == val.c;
 
-    var val_size := MarshallVal(val.val, grammar.cases[val.c], data, index + 8);
+  var val_size := MarshallVal(val.val, grammar.cases[val.c], data, index + 8);
 
-    ghost var new_int_bytes := data[index..index+Uint64Size()];
-    assert forall i {:auto_trigger} :: 0 <= i < Uint64Size() ==> int_bytes[i] == new_int_bytes[i];
-    assert int_bytes == new_int_bytes;
+  ghost var new_int_bytes := data[index..index+Uint64Size()];
+  assert forall i {:auto_trigger} :: 0 <= i < Uint64Size() ==> int_bytes[i] == new_int_bytes[i];
+  assert int_bytes == new_int_bytes;
 
-    assert val.VCase?; 
-    assert grammar.GTaggedUnion?; 
-    assert int(val.c) < |grammar.cases|;
+  assert val.VCase?; 
+  assert grammar.GTaggedUnion?; 
+  assert val.c as int < |grammar.cases|;
 
-    ghost var bytes := data[index..int(index) + SizeOfV(val)];
-    assert bytes[..8] == new_int_bytes;
-    calc {
-        parse_Val(bytes, grammar);
-            { reveal_parse_Val(); }
-        parse_Case(bytes, grammar.cases);
-    }
+  ghost var bytes := data[index..(index as int) + SizeOfV(val)];
+  assert bytes[..8] == new_int_bytes;
+  calc {
+    parse_Val(bytes, grammar);
+      { reveal parse_Val(); }
+    parse_Case(bytes, grammar.cases);
+  }
 
-    assert{:split_here} true;
-    ghost var tuple1 := parse_Uint64(bytes);
-    ghost var caseID := tuple1.0;
-    ghost var rest1   := tuple1.1;
+  assert{:split_here} true;
+  ghost var tuple1 := parse_Uint64(bytes);
+  ghost var caseID := tuple1.0;
+  ghost var rest1   := tuple1.1;
 
-    assert !caseID.None?;
-    assert caseID.v.u == val.c;
-    assert int(caseID.v.u) < |grammar.cases|;
-    ghost var tuple2 := parse_Val(rest1, grammar.cases[caseID.v.u]);
-    ghost var v:= tuple2.0;
-    ghost var rest2 := tuple2.1;
-    assert !v.None?;
+  assert !caseID.None?;
+  assert caseID.v.u == val.c;
+  assert (caseID.v.u as int) < |grammar.cases|;
+  ghost var tuple2 := parse_Val(rest1, grammar.cases[caseID.v.u]);
+  ghost var v:= tuple2.0;
+  ghost var rest2 := tuple2.1;
+  assert !v.None?;
 
-    size := 8 + val_size;
+  size := 8 + val_size;
 }
 
 method MarshallVUint64(val:V, grammar:G, data:array<byte>, index:uint64) returns (size:uint64)
-    requires data != null;
-    requires val.VUint64?;
-    requires ValidGrammar(grammar);
-    requires ValInGrammar(val, grammar);
-    requires int(index) + SizeOfV(val) <= data.Length;
-    requires 0 <= int(index) + SizeOfV(val) < 0x1_0000_0000_0000_0000;  // Needed to prevent overflow below
-    requires data.Length < 0x1_0000_0000_0000_0000;
-    modifies data;
-    decreases grammar;
-    ensures  parse_Val(data[index..int(index) + SizeOfV(val)], grammar).0.Some? &&
-             parse_Val(data[index..int(index) + SizeOfV(val)], grammar).0.v == val;
-    ensures  forall i :: 0 <= i < index ==> data[i] == old(data[i]);
-    ensures  forall i :: int(index) + SizeOfV(val) <= i < data.Length ==> data[i] == old(data[i]);
-    ensures  int(size) == SizeOfV(val);
+  requires val.VUint64?
+  requires ValidGrammar(grammar)
+  requires ValInGrammar(val, grammar)
+  requires (index as int) + SizeOfV(val) <= data.Length
+  requires 0 <= (index as int) + SizeOfV(val) < 0x1_0000_0000_0000_0000   // Needed to prevent overflow below
+  requires data.Length < 0x1_0000_0000_0000_0000
+  modifies data
+  decreases grammar
+  ensures  parse_Val(data[index..(index as int) + SizeOfV(val)], grammar).0.Some? &&
+           parse_Val(data[index..(index as int) + SizeOfV(val)], grammar).0.v == val
+  ensures  forall i :: 0 <= i < index ==> data[i] == old(data[i])
+  ensures  forall i :: (index as int) + SizeOfV(val) <= i < data.Length ==> data[i] == old(data[i])
+  ensures  size as int == SizeOfV(val)
 {
-    MarshallUint64(val.u, data, index);
-    calc {
-        parse_Val(data[index..int(index) + SizeOfV(val)], grammar);
-            { reveal_parse_Val(); }
-        parse_Uint64(data[index..int(index) + SizeOfV(val)]);
-    }
-    return 8;
+  MarshallUint64(val.u, data, index);
+  calc {
+    parse_Val(data[index..(index as int) + SizeOfV(val)], grammar);
+      { reveal parse_Val(); }
+    parse_Uint64(data[index..(index as int) + SizeOfV(val)]);
+  }
+  return 8;
 }
 
 method MarshallVal(val:V, grammar:G, data:array<byte>, index:uint64) returns (size:uint64)
-    requires ValidGrammar(grammar);
-    requires ValInGrammar(val, grammar);
-    requires ValidVal(val);
-    requires 0 <= SizeOfV(val) < 0x1_0000_0000_0000_0000;
-    requires data!=null;
-    requires int(index) + SizeOfV(val) <= data.Length;
-    requires data.Length < 0x1_0000_0000_0000_0000;
-    modifies data;
-    decreases grammar, 0;
-    ensures  parse_Val(data[index..int(index) + SizeOfV(val)], grammar).0.Some? &&
-             parse_Val(data[index..int(index) + SizeOfV(val)], grammar).0.v == val;
-    ensures  forall i :: 0 <= i < index ==> data[i] == old(data[i]);
-    ensures  forall i :: int(index) + SizeOfV(val) <= i < data.Length ==> data[i] == old(data[i]);
-    ensures  int(size) == SizeOfV(val);
+  requires ValidGrammar(grammar)
+  requires ValInGrammar(val, grammar)
+  requires ValidVal(val)
+  requires 0 <= SizeOfV(val) < 0x1_0000_0000_0000_0000
+  requires (index as int) + SizeOfV(val) <= data.Length
+  requires data.Length < 0x1_0000_0000_0000_0000
+  modifies data
+  decreases grammar, 0
+  ensures  parse_Val(data[index..(index as int) + SizeOfV(val)], grammar).0.Some? &&
+           parse_Val(data[index..(index as int) + SizeOfV(val)], grammar).0.v == val
+  ensures  forall i :: 0 <= i < index ==> data[i] == old(data[i])
+  ensures  forall i :: (index as int) + SizeOfV(val) <= i < data.Length ==> data[i] == old(data[i])
+  ensures  size as int == SizeOfV(val)
 {
-    match val
-        case VUint64(_)    => size := MarshallVUint64(val, grammar, data, index);
-        case VArray(_)     => size := MarshallArray(val, grammar, data, index);
-        case VTuple(_)     => size := MarshallTuple(val, grammar, data, index);
-        case VByteArray(_) => size := MarshallByteArray(val, grammar, data, index);
-        case VCase(_,_)    => size := MarshallCase(val, grammar, data, index);
+  match val
+    case VUint64(_)    => size := MarshallVUint64(val, grammar, data, index);
+    case VArray(_)     => size := MarshallArray(val, grammar, data, index);
+    case VTuple(_)     => size := MarshallTuple(val, grammar, data, index);
+    case VByteArray(_) => size := MarshallByteArray(val, grammar, data, index);
+    case VCase(_,_)    => size := MarshallCase(val, grammar, data, index);
 }
 
 method Marshall(val:V, grammar:G) returns (data:array<byte>)
-    requires ValidGrammar(grammar);
-    requires ValInGrammar(val, grammar);
-    requires ValidVal(val);
-    requires 0 <= SizeOfV(val) < 0x1_0000_0000_0000_0000;
-    ensures data!=null;
-    ensures fresh(data);
-    ensures Demarshallable(data[..], grammar);
-    ensures parse_Val(data[..], grammar).0.Some? && parse_Val(data[..], grammar).0.v == val;
-    ensures parse_Val(data[..], grammar).1 == [];
-    ensures |data[..]| == SizeOfV(val);
+  requires ValidGrammar(grammar)
+  requires ValInGrammar(val, grammar)
+  requires ValidVal(val)
+  requires 0 <= SizeOfV(val) < 0x1_0000_0000_0000_0000
+  ensures fresh(data)
+  ensures Demarshallable(data[..], grammar)
+  ensures parse_Val(data[..], grammar).0.Some? && parse_Val(data[..], grammar).0.v == val
+  ensures parse_Val(data[..], grammar).1 == []
+  ensures |data[..]| == SizeOfV(val)
 {
-    var size := ComputeSizeOf(val);
-    data := new byte[size];
+  var size := ComputeSizeOf(val);
+  data := new byte[size];
 
-    var computed_size := MarshallVal(val, grammar, data, 0);
+  var computed_size := MarshallVal(val, grammar, data, 0);
 
-    assert data[0..0 + SizeOfV(val)] == data[0..0 + size] == data[..];      // OBSERVE
+  assert data[0..0 + SizeOfV(val)] == data[0..0 + size] == data[..];      // OBSERVE
 
-    lemma_parse_Val_view_specific(data[..], val, grammar, 0, int(size));
+  lemma_parse_Val_view_specific(data[..], val, grammar, 0, size as int);
 }
+
 } 
