ironfleet/src/Dafny/Distributed/Impl/Common/MarshallInt.i.dfy
@@ -1,59 +1,58 @@
 include "../../Common/Native/NativeTypes.s.dfy"
-//include "../../../Libraries/Util/seqs_transforms.i.dfy"
 include "Util.i.dfy"
 
 module Common__MarshallInt_i {
 import opened Native__NativeTypes_s
-//import opened Util__seqs_transforms_i
+import opened Native__NativeTypes_i
 import opened Common__Util_i
+import opened Math__power2_i
 
 /*  Doesn't appear to be in use at present
 method MarshallUint32_guts(n:uint32, data:array<byte>, index:uint64)
-    requires data != null;
-    requires int(index) + int(Uint32Size()) <= data.Length;
-    requires 0 <= int(index) + int(Uint32Size()) < 0x1_0000_0000_0000_0000;  // Needed to prevent overflow on the next line
-    requires data.Length < 0x1_0000_0000_0000_0000;
-    modifies data;
-    ensures  BEByteSeqToUint32(data[index..index+uint64(Uint32Size())]) == n;
-    ensures  data[0..index] == old(data[0..index]);
-    ensures  data[index+uint64(Uint32Size())..] == old(data[index+uint64(Uint32Size())..]);
+  requires data != null
+  requires (index as int) + (Uint32Size() as int) <= data.Length
+  requires 0 <= (index as int) + (Uint32Size() as int) < 0x1_0000_0000_0000_0000  // Needed to prevent overflow on the next line
+  requires data.Length < 0x1_0000_0000_0000_0000
+  modifies data
+  ensures  BEByteSeqToUint32(data[index..index+uint64(Uint32Size())]) == n
+  ensures  data[0..index] == old(data[0..index])
+  ensures  data[index+uint64(Uint32Size())..] == old(data[index+uint64(Uint32Size())..])
 {
-    data[index  ] := byte( n/0x1000000);
-    data[index+1] := byte((n/  0x10000)%0x100);
-    data[index+2] := byte((n/    0x100)%0x100);
-    data[index+3] := byte( n           %0x100);
-    ghost var i := int(n);
-    ghost var bs := [ i / 16777216, (i / 65536) % 256, (i / 256) % 256, i % 256 ];
-    assert SeqByteToByteSeq(data[index..index+4]) == bs;
+  data[index  ] := ( n/0x1000000) as byte;
+  data[index+1] := ((n/  0x10000)%0x100) as byte;
+  data[index+2] := ((n/    0x100)%0x100) as byte;
+  data[index+3] := ( n           %0x100) as byte;
+  ghost var i := n as int;
+  ghost var bs := [ i / 16777216, (i / 65536) % 256, (i / 256) % 256, i % 256 ];
+  assert SeqByteToByteSeq(data[index..index+4]) == bs;
 
-    lemma_2toX();
-    BEWordToByte_literal(int(n), bs);
+  lemma_2toX();
+  BEWordToByte_literal(n as int, bs);
 }
 */
 
 method MarshallUint64_guts(n:uint64, data:array<byte>, index:uint64)
-    requires data != null;
-    requires int(index) + int(Uint64Size()) <= data.Length;
-    requires 0 <= int(index) + int(Uint64Size()) < 0x1_0000_0000_0000_0000;  // Needed to prevent overflow on the next line
-    requires data.Length < 0x1_0000_0000_0000_0000;
-    modifies data;
-    ensures  SeqByteToUint64(data[index..index+uint64(Uint64Size())]) == n;
-    ensures  data[0..index] == old(data[0..index]);
-    ensures  data[index+uint64(Uint64Size())..] == old(data[index+uint64(Uint64Size())..]);
+  requires (index as int) + (Uint64Size() as int) <= data.Length
+  requires 0 <= (index as int) + (Uint64Size() as int) < 0x1_0000_0000_0000_0000  // Needed to prevent overflow on the next line
+  requires data.Length < 0x1_0000_0000_0000_0000
+  modifies data
+  ensures  SeqByteToUint64(data[index..index+(Uint64Size() as uint64)]) == n
+  ensures  data[0..index] == old(data[0..index])
+  ensures  data[index+(Uint64Size() as uint64)..] == old(data[index+(Uint64Size() as uint64)..])
 {
-    data[index  ] := byte( n/0x1000000_00000000);
-    data[index+1] := byte((n/  0x10000_00000000)%0x100);
-    data[index+2] := byte((n/    0x100_00000000)%0x100);
-    data[index+3] := byte((n/      0x1_00000000)%0x100);
-    data[index+4] := byte((n/         0x1000000)%0x100);
-    data[index+5] := byte((n/           0x10000)%0x100);
-    data[index+6] := byte((n/             0x100)%0x100);
-    data[index+7] := byte( n                    %0x100);
+  data[index  ] :=  (n/0x1000000_00000000)        as byte;
+  data[index+1] := ((n/  0x10000_00000000)%0x100) as byte;
+  data[index+2] := ((n/    0x100_00000000)%0x100) as byte;
+  data[index+3] := ((n/      0x1_00000000)%0x100) as byte;
+  data[index+4] := ((n/         0x1000000)%0x100) as byte;
+  data[index+5] := ((n/           0x10000)%0x100) as byte;
+  data[index+6] := ((n/             0x100)%0x100) as byte;
+  data[index+7] := ( n                    %0x100) as byte;
 
-    lemma_2toX();
+  lemma_2toX();
 
-    assert data[index..index+uint64(Uint64Size())] == Uint64ToSeqByte(n);
-    lemma_BEUintToSeqByte_invertability(data[index..index+uint64(Uint64Size())], int(n), 8);
+  assert data[index..index+(Uint64Size() as uint64)] == Uint64ToSeqByte(n);
+  lemma_BEUintToSeqByte_invertability(data[index..index+(Uint64Size() as uint64)], n as int, 8);
 }
 
 
