ironfleet/src/Dafny/Distributed/Impl/Common/UpperBound.i.dfy
@@ -7,20 +7,20 @@ import opened Native__NativeTypes_s
 import opened Common__UpperBound_s
 
 method UpperBoundedAdditionImpl(x:uint64, y:uint64, u:uint64) returns (sum:uint64)
-    ensures int(sum) == UpperBoundedAddition(int(x), int(y), UpperBoundFinite(int(u)));
+  ensures sum as int == UpperBoundedAddition(x as int, y as int, UpperBoundFinite(u as int));
 {
-    if y >= u
-    {
-        sum := u;
-    }
-    else if x >= u - y
-    {
-        sum := u;
-    }
-    else
-    {
-        sum := x + y;
-    }
+  if y >= u
+  {
+    sum := u;
+  }
+  else if x >= u - y
+  {
+    sum := u;
+  }
+  else
+  {
+    sum := x + y;
+  }
 }
 
 }
